@prefix : <http://vocab.gtfs.org/terms#> .
@prefix cc: <http://creativecommons.org/ns#> .
@prefix dct: <http://purl.org/dc/terms/> .
@prefix owl: <http://www.w3.org/2002/07/owl#> .
@prefix rdf: <http://www.w3.org/1999/02/22-rdf-syntax-ns#> .
@prefix xml: <http://www.w3.org/XML/1998/namespace> .
@prefix xsd: <http://www.w3.org/2001/XMLSchema#> .
@prefix adms: <http://www.w3.org/ns/adms#> .
@prefix dcat: <http://www.w3.org/ns/dcat#> .
@prefix foaf: <http://xmlns.com/foaf/0.1/> .
@prefix gtfs: <http://vocab.gtfs.org/terms#> .
@prefix rdfs: <http://www.w3.org/2000/01/rdf-schema#> .
@prefix skos: <http://www.w3.org/2004/02/skos/core#> .
@prefix vann: <http://purl.org/vocab/vann/> .
@prefix schema: <http://schema.org/> .
@prefix status: <http://www.w3.org/2003/06/sw-vocab-status/ns#> .
@prefix transit: <http://vocab.org/transit/terms/> .
@prefix geo: <http://www.w3.org/2003/01/geo/wgs84_pos#> .
@base <http://vocab.gtfs.org/terms#> .

<http://vocab.gtfs.org/terms#> rdf:type owl:Ontology ;
                                dct:creator [ foaf:mbox "Pieter.Colpaert@UGent.be" ;
                                              foaf:name "Pieter Colpaert"
                                            ] ,
                                            [ foaf:mbox "abyrd@conveyal.com" ;
                                              foaf:name "Andrew Byrd"
                                            ] ;
                                dct:description "Esta ontología es una traducción de la Especificación General de Feeds de Transporte Público a URIs. El objetivo es crear una plataforma de intercambio donde el modelo Linked GTFS pueda usarse para obtener los datos correctos en el formato adecuado. Para la especificación semántica de clases y propiedades, visite https://developers.google.com/transit/gtfs/reference."@es ,
                                                "This ontology is a translation of the General Transit Feed Specification towards URIs. Its intended use is creating an exchange platform where the Linked GTFS model can be used as a start to get the right data into the right format. For semantics of the classes and properties, see https://developers.google.com/transit/gtfs/reference."@en ;
                                vann:preferredNamespacePrefix "gtfs" ;
                                vann:preferredNamespaceUri "http://vocab.gtfs.org/terms#" ;
                                rdfs:label "Especificación General de Feeds de Transporte Público"@es ,
                                           "General Transit Feed Specification"@en ;
                                rdfs:seeAlso <https://developers.google.com/transit/gtfs/reference> .

#################################################################
#    Annotation properties
#################################################################

###  http://creativecommons.org/ns#license
cc:license rdf:type owl:AnnotationProperty .


###  http://purl.org/dc/terms/creator
dct:creator rdf:type owl:AnnotationProperty .


###  http://purl.org/dc/terms/description
dct:description rdf:type owl:AnnotationProperty .


###  http://purl.org/dc/terms/hasFormat
dct:hasFormat rdf:type owl:AnnotationProperty .


###  http://purl.org/dc/terms/issued
dct:issued rdf:type owl:AnnotationProperty .


###  http://purl.org/dc/terms/modified
dct:modified rdf:type owl:AnnotationProperty .


###  http://purl.org/dc/terms/rights
dct:rights rdf:type owl:AnnotationProperty .


###  http://purl.org/dc/terms/title
dct:title rdf:type owl:AnnotationProperty .


###  http://purl.org/vocab/vann/preferredNamespacePrefix
vann:preferredNamespacePrefix rdf:type owl:AnnotationProperty .


###  http://purl.org/vocab/vann/preferredNamespaceUri
vann:preferredNamespaceUri rdf:type owl:AnnotationProperty .


###  http://vocab.gtfs.org/terms#comment
gtfs:comment rdfs:comment "A comment on the relation between the RDFS ontology and the CSV specification."@en ,
                          "Un comentario entre la relación entre la ontología RDFS y la especificación CSV."@es ;
             rdfs:label "Comentario de enlace"@es ,
                        "Mapping comment"@en ;
             status:term_status "inestable"@es ,
                                "unstable"@en ;
             rdf:type owl:AnnotationProperty ;
             rdfs:subPropertyOf rdfs:comment .

###  http://www.w3.org/2003/06/sw-vocab-status/ns#term_status
status:term_status rdf:type owl:AnnotationProperty .


###  http://www.w3.org/ns/adms#versionNotes
adms:versionNotes rdf:type owl:AnnotationProperty .


###  http://www.w3.org/ns/dcat#theme
dcat:theme rdf:type owl:AnnotationProperty .


###  http://xmlns.com/foaf/0.1/mbox
foaf:mbox rdf:type owl:AnnotationProperty .


###  http://xmlns.com/foaf/0.1/name
foaf:name rdf:type owl:AnnotationProperty .


###  http://xmlns.com/foaf/0.1/page
foaf:page rdf:type owl:AnnotationProperty .


###  http://xmlns.com/foaf/0.1/primaryTopic
foaf:primaryTopic rdf:type owl:AnnotationProperty .


#################################################################
#    Datatypes
#################################################################

###  http://www.w3.org/2001/XMLSchema#date
xsd:date rdf:type rdfs:Datatype .


###  http://www.w3.org/2001/XMLSchema#duration
xsd:duration rdf:type rdfs:Datatype .


#################################################################
#    Object Properties
#################################################################

###  http://vocab.gtfs.org/terms#agency
gtfs:agency rdf:type owl:ObjectProperty ;
            rdfs:domain gtfs:Route ;
            rdfs:range gtfs:Agency ;
            rdfs:comment "Enlaza a una agencia de la que este concepto es parte."@es ,
                         "links to an agency that this is part of."@en ;
            rdfs:label "agency"@en ,
                       "empresa"@es ;
            status:term_status "inestable"@es ,
                               "unstable"@en .


###  http://vocab.gtfs.org/terms#block
gtfs:block rdf:type owl:ObjectProperty ;
           rdfs:domain gtfs:Trip ;
           rdfs:range gtfs:Block ;
           rdfs:comment "Identifica el bloque al que pertenece el viaje. Un bloque consta de dos o más viajes secuenciales realizados en el mismo vehículo, en los que un pasajero puede cambiar de viaje si simplemente permanece en el vehículo."@es ,
                        "Identifies the block to which the trip within this feed belongs. A block consists of two or more sequential trips made using the same vehicle, where a passenger can transfer from one trip to the next just by staying in the vehicle."@en ;
           rdfs:label "Block"@en ,
                      "Bloque"@es ;
           status:term_status "inestable"@es ,
                              "unstable"@en .


###  http://vocab.gtfs.org/terms#containsZone
gtfs:containsZone rdf:type owl:ObjectProperty ;
                  rdfs:domain gtfs:FareRule ;
                  rdfs:range gtfs:Zone ;
                  rdfs:comment "Identifies the zones that a rider will enter while using a given fare class. Used in some systems to calculate correct fare class."@en ;
                  rdfs:label "Contains Zone"@en .


###  http://vocab.gtfs.org/terms#continuousDropOffType
gtfs:continuousDropOffType rdf:type owl:ObjectProperty ;
                           rdfs:range gtfs:ContinuousDropOff ;
                           rdfs:comment "Indicates whether a rider can alight from the transit vehicle at any point along the vehicle’s travel path."@en ;
                           rdfs:label "Continuous Drop Off Type"@en .


###  http://vocab.gtfs.org/terms#continuousPickupType
gtfs:continuousPickupType rdf:type owl:ObjectProperty ;
                          rdfs:range gtfs:ContinuousPickup ;
                          rdfs:comment "Indicates whether a rider can board the transit vehicle at any point along the vehicle’s travel path."@en ;
                          rdfs:label "Continuous Pickup Type"@en .


###  http://vocab.gtfs.org/terms#destination
gtfs:destination rdf:type owl:ObjectProperty ;
                 rdfs:domain gtfs:FareRule ;
                 rdfs:range gtfs:Zone ;
                 rdfs:comment "Identifies a destination zone."@en ;
                 rdfs:label "Destination"@en .


###  http://vocab.gtfs.org/terms#destinationStop
gtfs:destinationStop rdf:type owl:ObjectProperty ;
                     rdfs:range gtfs:Stop ;
                     gtfs:comment "Conectado a to_stop_id en transfers.txt"@es ,
                                  "Map from to_stop_id in transfers.txt"@en ;
                     rdfs:comment "Enlace al gtfs:Stop hacia el que va el viaje"@es ,
                                  "Link to gtfs:Stop to go to"@en ;
                     rdfs:label "Destination Stop"@en ,
                                "parada de destino"@es ;
                     status:term_status "inestable"@es ,
                                        "unstable"@en .


###  http://vocab.gtfs.org/terms#dropOffType
gtfs:dropOffType rdf:type owl:ObjectProperty ;
                 rdfs:range [ owl:intersectionOf ( <http://www.w3.org/2004/02/skos/core#Concept>
                                                  [ rdf:type owl:Restriction ;
                                                    owl:onProperty <http://www.w3.org/2004/02/skos/core#inScheme> ;
                                                    owl:hasValue <http://transport.linkeddata.es/kos/drop-off> ;
                                                  ]
                                                ) ;
                             rdf:type owl:Class
                            ] ;
                 rdfs:comment "Indica si los pasajeros se bajan en una parada como parte del horario normal o si no pueden bajar en esa parada."@es ,
                              "Indicates drop off method."@en ;
                 rdfs:label "Drop off type"@en ,
                            "tipo de bajada"@es ;
                 status:term_status "inestable"@es ,
                                    "unstable"@en .


gtfs:continuousDropOff rdf:type owl:ObjectProperty ;
                       rdfs:range [ owl:intersectionOf ( <http://www.w3.org/2004/02/skos/core#Concept>
                                                        [ rdf:type owl:Restriction ;
                                                          owl:onProperty <http://www.w3.org/2004/02/skos/core#inScheme> ;
                                                          owl:hasValue <http://transport.linkeddata.es/kos/drop-off> ;
                                                        ]
                                                     ) ;
                                    rdf:type owl:Class
                                ] ;
                       rdfs:comment "Indica si se bajan los pasajeros en cualquier punto del trayecto del vehículo."@es ,
                                    "Indicates that the rider can alight the transit vehicle at any point along the vehicle’s travel path."@en ;
                       rdfs:label "Continuous Drop Off"@en ,
                                  "Bajada continua"@es.


###  http://vocab.gtfs.org/terms#fare
gtfs:fare rdf:type owl:ObjectProperty ;
          rdfs:domain gtfs:FareRule ;
          rdfs:range gtfs:FareClass ;
          rdfs:comment "Identifies a fare class."@en ;
          rdfs:label "Fare"@en .


###  http://vocab.gtfs.org/terms#level
gtfs:level rdf:type owl:ObjectProperty ;
           rdfs:domain gtfs:Location ;
           rdfs:range gtfs:Level ;
           rdfs:comment "Identifies the level of the location."@en ;
           rdfs:label "Level"@en .


###  http://vocab.gtfs.org/terms#origin
gtfs:origin rdf:type owl:ObjectProperty ;
            rdfs:domain gtfs:FareRule ;
            rdfs:range gtfs:Zone ;
            rdfs:comment "Identifies an origin zone."@en ;
            rdfs:label "Origin"@en .


###  http://vocab.gtfs.org/terms#originStop
gtfs:originStop rdf:type owl:ObjectProperty ;
                rdfs:range gtfs:Stop ;
                gtfs:comment "Conectado a from_stop_id en transfers.txt"@es ,
                             "Map from from_stop_id in transfers.txt"@en ;
                rdfs:comment "Enlace al gtfs:Stop desde el que empieza el viaje"@es ,
                             "Link to gtfs:Stop to start from"@en ;
                rdfs:label "Origin Stop"@en ,
                           "parada de origen"@es ;
                status:term_status "inestable"@es ,
                                   "unstable"@en .


###  http://vocab.gtfs.org/terms#parentStation
gtfs:parentStation rdf:type owl:ObjectProperty ;
                   rdfs:domain gtfs:Stop ;
                   rdfs:range gtfs:Station ;
                   rdfs:comment "gtfs:parentStation defines hierarchy between the different locations"@en ,
                                "gtfs:parentStation identifica la estación asociada a la parada"@es ;
                   rdfs:label "Parent Station"@en ,
                              "estación matriz"@es ;
                   status:term_status "inestable"@es ,
                                      "unstable"@en .


###  http://vocab.gtfs.org/terms#pathwayMode
gtfs:pathwayMode rdf:type owl:ObjectProperty ;
                 rdfs:domain gtfs:Pathway ;
                 rdfs:range [ rdf:type owl:Class ;
                              owl:unionOf ( gtfs:Elevator 
                                            gtfs:Escalator
                                            gtfs:ExitGate
                                            gtfs:FareGate
                                            gtfs:MovingSidewalk
                                            gtfs:Stairs
                                            gtfs:Walkway 
                                          )
                            ] ;
                 rdfs:comment "Type of pathway between the specified gtfs:originStop and gtfs:destinationStop pair."@en ;
                 rdfs:label "Pathway Mode"@en .


###  http://vocab.gtfs.org/terms#paymentMethod
gtfs:paymentMethod rdf:type owl:ObjectProperty ;
                   rdfs:domain gtfs:FareClass ;
                   rdfs:range gtfs:PaymentMethod ;
                   gtfs:comment "Campo payment_method en fare_attributes. Si es 0, use gtfs:OnBoard; si es 1, use gtfs:BeforeBoarding"@es ,
                                "payment_method field in fare_attributes. If 0, use gtfs:OnBoard; if 1, use gtfs:BeforeBoarding"@en ;
                   rdfs:comment "The payment method"@en ,
                                "el método de pago"@es ;
                   rdfs:label "Método de pago"@es ,
                              "Payment method"@en ;
                   status:term_status "inestable"@es ,
                                      "unstable"@en .


###  http://vocab.gtfs.org/terms#pickupType
gtfs:pickupType rdf:type owl:ObjectProperty ;
                rdfs:range [ owl:intersectionOf ( <http://www.w3.org/2004/02/skos/core#Concept>
                                                  [ rdf:type owl:Restriction ;
                                                    owl:onProperty <http://www.w3.org/2004/02/skos/core#inScheme> ;
                                                    owl:hasValue <http://transport.linkeddata.es/kos/pickup> ;
                                                  ]
                                                ) ;
                             rdf:type owl:Class
                            ] ;
                rdfs:comment "Indica si se recogen los pasajeros en una parada como parte del horario normal o si su recogida en dicha parada no se encuentra disponible."@es ,
                             "Indicates pickup method."@en ;
                rdfs:label "Pickup type"@en ,
                           "tipo de recogida"@es ;
                status:term_status "inestable"@es ,
                                   "unstable"@en .


gtfs:continuousPickup rdf:type owl:ObjectProperty ;
                      rdfs:range [ owl:intersectionOf ( <http://www.w3.org/2004/02/skos/core#Concept>
                                                        [ rdf:type owl:Restriction ;
                                                          owl:onProperty <http://www.w3.org/2004/02/skos/core#inScheme> ;
                                                          owl:hasValue <http://transport.linkeddata.es/kos/pickup> ;
                                                        ]
                                                     ) ;
                                    rdf:type owl:Class
                                ] ;
                      rdfs:comment "Indica si se recogen los pasajeros en cualquier punto del trayecto del vehículo."@es ,
                                   "Indicates that the rider can board the transit vehicle at any point along the vehicle’s travel path."@en ;
                      rdfs:label "Continuous Pickup"@en ,
                                 "Recogida continua"@es.


###  http://vocab.gtfs.org/terms#route
gtfs:route rdf:type owl:ObjectProperty ;
           rdfs:domain gtfs:Trip ;
           rdfs:range [ rdf:type owl:Class ;
                        owl:unionOf ( gtfs:FareRule
                                      gtfs:Route
                                    )
                      ] ;
           rdfs:comment "Este viaje forma parte de esta gtfs:Route"@es ,
                        "This thing is applicable to this gtfs:Route"@en ;
           rdfs:label "Route"@en ,
                      "ruta"@es ;
           status:term_status "inestable"@es ,
                              "unstable"@en .


###  http://vocab.gtfs.org/terms#routeType
gtfs:routeType rdf:type owl:ObjectProperty ;
               rdfs:domain gtfs:Route ;
               rdfs:range [ owl:intersectionOf ( <http://www.w3.org/2004/02/skos/core#Concept>
                                                 [ rdf:type owl:Restriction ;
                                                   owl:onProperty <http://www.w3.org/2004/02/skos/core#inScheme> ;
                                                   owl:hasValue <http://transport.linkeddata.es/kos/route-type> ;
                                                  ]
                                               ) ;
                            rdf:type owl:Class
                          ] ;
               rdfs:comment "Enlaza al tipo de vehículo que opera en esta ruta"@es ,
                            "Indicates the type of transportation used on a route."@en ;
               rdfs:label "Route type"@en ,
                          "tipo de ruta"@es ;
               rdfs:seeAlso <https://developers.google.com/transit/gtfs/examples/display-to-users#RouteType> ;
               status:term_status "inestable"@es ,
                                  "unstable"@en .


###  http://vocab.gtfs.org/terms#service
gtfs:service rdf:type owl:ObjectProperty ;
             rdfs:range gtfs:Service ;
             rdfs:comment "Cumple este gtfs:Service."@es ,
                          "Identifies a set of dates when service is available for one or more routes."@en ;
             rdfs:label "Service"@en ,
                        "Servicio"@es ;
             status:term_status "inestable"@es ,
                                "unstable"@en .


###  http://vocab.gtfs.org/terms#serviceRule
gtfs:serviceRule rdfs:comment "Reglas de servicio que definen un conjunto de fechas"@es ,
                              "Service rules which define together a set of dates"@en ;
                 rdfs:label "Service rule"@en ,
                            "regla de servicio"@es ;
                 status:term_status "inestable"@es ,
                                    "unstable"@en ;
                 rdf:type owl:ObjectProperty ;
                 rdfs:domain gtfs:Service ;
                 rdfs:range gtfs:ServiceRule .


###  http://vocab.gtfs.org/terms#shape
gtfs:shape rdf:type owl:ObjectProperty ;
           rdfs:domain gtfs:Trip ;
           rdfs:range gtfs:Shape ;
           rdfs:comment "Identifies a geospatial shape that describes the vehicle travel path for a trip."@en ,
                        "Un enlace al recorrido que sigue el viaje."@es ;
           rdfs:label "Shape"@en ,
                      "forma del recorrido, trayecto, itinerario"@es ;
           status:term_status "inestable"@es ,
                              "unstable"@en .


###  http://vocab.gtfs.org/terms#shapePoint
gtfs:shapePoint rdf:type owl:ObjectProperty ;
                rdfs:domain gtfs:Shape ;
                rdfs:range gtfs:ShapePoint ;
                rdfs:comment "Enlaza a gtfs:ShapePoint"@es ,
                             "Links to a gtfs:ShapePoint"@en ;
                rdfs:label "Shape Point"@en ,
                           "punto de recorrido"@es ;
                status:term_status "inestable"@es ,
                                   "unstable"@en .


###  http://vocab.gtfs.org/terms#stop
gtfs:stop rdf:type owl:ObjectProperty ;
          rdfs:domain gtfs:StopTime ;
          rdfs:range gtfs:Stop ;
          rdfs:comment "Indica que este concepto tiene cierta parada."@es ,
                       "Indicates that this has a certain stop."@en ;
          rdfs:label "Stop"@en ,
                     "parada"@es ;
          status:term_status "inestable"@es ,
                             "unstable"@en .


###  http://vocab.gtfs.org/terms#transferType
gtfs:transferType rdf:type owl:ObjectProperty ;
                  rdfs:domain gtfs:Transfer ;
                  rdfs:range gtfs:TransferType ;
                  rdfs:comment "Indicates the type of connection between the specified gtfs:originStop and gtfs:destinationStop pair."@en ;
                  rdfs:label "Transfer Type"@en ,
                             "tipo de transbordo"@es ;
                  status:term_status "inestable"@es ,
                                     "unstable"@en .


###  http://vocab.gtfs.org/terms#transfers
gtfs:transfers rdf:type owl:ObjectProperty ;
               rdfs:domain gtfs:FareClass ;
               rdfs:range gtfs:TransfersAllowedType ;
               gtfs:comment "Map to 0 to gtfs:NoTransfersAllowed, 1 to gtfs:OneTransferAllowed, 2 to gtfs:TwoTransfersAllowed and empty to gtfs:UnlimitedTransfersAllowed"@en ,
                            "Valor 0 si no se permite ningún transbordo (gtfs:NoTransfersAllowed), 1 si se puede realizar un transbordo (gtfs:OneTransferAllowed), 2 si se pueden realizar dos transbordos (gtfs:TwoTransfersAllowed) y deje el campo vacío si se permite una cantidad ilimitada de transbordos (gtfs:UnlimitedTransfersAllowed)"@es ;
               rdfs:comment "The validity of the ticket when transferring"@en ,
                            "Validez del ticket para transbordos"@es ;
               rdfs:label "Transfers"@en ,
                          "transbordos"@es ;
               status:term_status "inestable"@es ,
                                  "unstable"@en .


###  http://vocab.gtfs.org/terms#trip
gtfs:trip rdf:type owl:ObjectProperty ;
          rdfs:domain [ rdf:type owl:Class ;
                        owl:unionOf ( gtfs:StopTime 
                                      gtfs:Frequency 
                                    )
                      ] ;
          rdfs:range gtfs:Trip ;
          rdfs:comment "Indica que este concepto es parte de cierto gtfs:Trip"@es ,
                       "Indicates that this is part of a certain gtfs:Trip"@en ;
          rdfs:label "Trip"@en ,
                     "viaje"@es ;
          status:term_status "inestable"@es ,
                             "unstable"@en .


###  http://vocab.gtfs.org/terms#zone
gtfs:zone rdf:type owl:ObjectProperty ;
          rdfs:range gtfs:Zone ;
          gtfs:comment "Puede crear una nueva URI por zona, o simplemente referenciarla con un número entero."@es ,
                       "You can create a new URI per zone, or just keep it an integer as per your own taste."@en ;
          rdfs:comment "A gtfs:Stop defines the fare zone. Zones are required if you want to provide fare information using gtfs:FareClass."@en ,
                       "Un gtfs:Stop define la zona tarifaria. Las zonas son necesarias si quiere proporcionar información de tarifas usando gtfs:FareClass."@es ;
          rdfs:label "Zone"@en ,
                     "zona"@es ;
          status:term_status "inestable"@es ,
                             "unstable"@en .


###  http://vocab.gtfs.org/terms#monday
gtfs:monday rdf:type owl:ObjectProperty ;
            rdfs:domain gtfs:CalendarRule ;
            rdfs:range [ owl:intersectionOf ( <http://www.w3.org/2004/02/skos/core#Concept>
                                              [ rdf:type owl:Restriction ;
                                                owl:onProperty <http://www.w3.org/2004/02/skos/core#inScheme> ;
                                                owl:hasValue <http://transport.linkeddata.es/kos/day> ;
                                              ]
                                            ) ;
                         rdf:type owl:Class
                        ] ;
            rdfs:comment "Service is available on all Mondays in the duration of the service calendar."@en ,
                         "Servicio disponible los lunes"@es ;
            rdfs:label "Monday"@en ,
                       "lunes"@es ;
            status:term_status "inestable"@es ,
                               "unstable"@en .


###  http://vocab.gtfs.org/terms#tuesday
gtfs:tuesday rdf:type owl:ObjectProperty ;
             rdfs:domain gtfs:CalendarRule ;
             rdfs:range [ owl:intersectionOf ( <http://www.w3.org/2004/02/skos/core#Concept>
                                              [ rdf:type owl:Restriction ;
                                                owl:onProperty <http://www.w3.org/2004/02/skos/core#inScheme> ;
                                                owl:hasValue <http://transport.linkeddata.es/kos/day> ;
                                              ]
                                            ) ;
                         rdf:type owl:Class
                        ] ;
             rdfs:comment "Service is available on all Tuesdays in the duration of the service calendar."@en ,
                          "Servicio disponible los martes"@es ;
             rdfs:label "Tuesday"@en ,
                        "martes"@es ;
             status:term_status "inestable"@es ,
                                "unstable"@en .


###  http://vocab.gtfs.org/terms#wednesday
gtfs:wednesday rdf:type owl:ObjectProperty ;
               rdfs:domain gtfs:CalendarRule ;
               rdfs:range [ owl:intersectionOf ( <http://www.w3.org/2004/02/skos/core#Concept>
                                              [ rdf:type owl:Restriction ;
                                                owl:onProperty <http://www.w3.org/2004/02/skos/core#inScheme> ;
                                                owl:hasValue <http://transport.linkeddata.es/kos/day> ;
                                              ]
                                            ) ;
                         rdf:type owl:Class
                        ] ;
               rdfs:comment "Service is available on all Wednesdays in the duration of the service calendar."@en ,
                            "Servicio disponible los miércoles"@es ;
               rdfs:label "Wednesday"@en ,
                          "miércoles"@es ;
               status:term_status "inestable"@es ,
                                  "unstable"@en .


###  http://vocab.gtfs.org/terms#thursday
gtfs:thursday rdf:type owl:ObjectProperty ;
              rdfs:domain gtfs:CalendarRule ;
              rdfs:range [ owl:intersectionOf ( <http://www.w3.org/2004/02/skos/core#Concept>
                                              [ rdf:type owl:Restriction ;
                                                owl:onProperty <http://www.w3.org/2004/02/skos/core#inScheme> ;
                                                owl:hasValue <http://transport.linkeddata.es/kos/day> ;
                                              ]
                                            ) ;
                         rdf:type owl:Class
                        ] ;
              rdfs:comment "Service is available on all Thursdays in the duration of the service calendar."@en ,
                           "Servicio disponible los jueves"@es ;
              rdfs:label "Thursday"@en ,
                         "jueves"@es ;
              status:term_status "inestable"@es ,
                                 "unstable"@en .


###  http://vocab.gtfs.org/terms#friday
gtfs:friday rdf:type owl:ObjectProperty ;
            rdfs:domain gtfs:CalendarRule ;
            rdfs:range [ owl:intersectionOf ( <http://www.w3.org/2004/02/skos/core#Concept>
                                              [ rdf:type owl:Restriction ;
                                                owl:onProperty <http://www.w3.org/2004/02/skos/core#inScheme> ;
                                                owl:hasValue <http://transport.linkeddata.es/kos/day> ;
                                              ]
                                            ) ;
                         rdf:type owl:Class
                        ] ;
            rdfs:comment "Service is available on all Fridays in the duration of the service calendar."@en ,
                         "Servicio disponible los viernes"@es ;
            rdfs:label "Friday"@en ,
                       "viernes"@es ;
            status:term_status "inestable"@es ,
                               "unstable"@en .


###  http://vocab.gtfs.org/terms#saturday
gtfs:saturday rdf:type owl:ObjectProperty ;
              rdfs:domain gtfs:CalendarRule ;
              rdfs:range [ owl:intersectionOf ( <http://www.w3.org/2004/02/skos/core#Concept>
                                              [ rdf:type owl:Restriction ;
                                                owl:onProperty <http://www.w3.org/2004/02/skos/core#inScheme> ;
                                                owl:hasValue <http://transport.linkeddata.es/kos/day> ;
                                              ]
                                            ) ;
                         rdf:type owl:Class
                        ] ;
              rdfs:comment "Service is available on all Saturdays in the duration of the service calendar."@en ,
                           "Servicio disponible los sábados"@es ;
              rdfs:label "Saturday"@en ,
                         "sábado"@es ;
              status:term_status "inestable"@es ,
                                 "unstable"@en .


###  http://vocab.gtfs.org/terms#sunday
gtfs:sunday rdf:type owl:ObjectProperty ;
            rdfs:domain gtfs:CalendarRule ;
            rdfs:range [ owl:intersectionOf ( <http://www.w3.org/2004/02/skos/core#Concept>
                                              [ rdf:type owl:Restriction ;
                                                owl:onProperty <http://www.w3.org/2004/02/skos/core#inScheme> ;
                                                owl:hasValue <http://transport.linkeddata.es/kos/day> ;
                                              ]
                                            ) ;
                         rdf:type owl:Class
                        ] ;
            rdfs:comment "Service is available on all Sundays in the duration of the service calendar."@en ,
                         "Servicio disponible los domingos"@es ;
            rdfs:label "Sunday"@en ,
                       "domingos"@es ;
            status:term_status "inestable"@es ,
                               "unstable"@en .


gtfs:exceptionType rdf:type owl:ObjectProperty ;
                   rdfs:domain gtfs:CalendarDateRule ;
                   rdfs:range [ owl:intersectionOf ( <http://www.w3.org/2004/02/skos/core#Concept>
                                                      [ rdf:type owl:Restriction ;
                                                        owl:onProperty <http://www.w3.org/2004/02/skos/core#inScheme> ;
                                                        owl:hasValue <http://transport.linkeddata.es/kos/exception-type> ;
                                                      ]
                                                    ) ;
                                rdf:type owl:Class
                              ] ;
                   rdfs:comment "Indicates whether service is available on the date specified in the date field. Valid options are: 1 - Service has been added for the specified date. 2 - Service has been removed for the specified date."@en ;
                   rdfs:label "Exception Type"@en .


###  http://vocab.gtfs.org/terms#usesExactTimes
gtfs:usesExactTimes rdf:type owl:ObjectProperty ;
                    rdfs:domain gtfs:Frequency ;
                    rdfs:range [ owl:intersectionOf ( <http://www.w3.org/2004/02/skos/core#Concept>
                                              [ rdf:type owl:Restriction ;
                                                owl:onProperty <http://www.w3.org/2004/02/skos/core#inScheme> ;
                                                owl:hasValue <http://transport.linkeddata.es/kos/exact-times> ;
                                              ]
                                            ) ;
                         rdf:type owl:Class
                        ] ;
                    gtfs:comment "Determina si los viajes basados en frecuencias deben estar programados de manera exacta según la información especificada de tiempo entre viajes. Falso cuando exact_times es 0 (o vacío), verdadero cuando es uno 1"@es ,
                                 "Indicates the type of service for a trip. [0 or empty - Frequency-based trips. - Frequency-based service (exact_times=0) in which service does not follow a fixed schedule throughout the day. Instead, operators attempt to strictly maintain predetermined headways for trips., 1 - Schedule-based trips with the exact same headway throughout the day. has the exact same headway for trips over specified time period(s). In schedule-based service operators try to strictly adhere to a schedule.]"@en ;
                    rdfs:label "Frequency uses exact times"@en ,
                               "Viajes basados en frecuencias programados de manera exacta"@es ;
                    status:term_status "inestable"@es ,
                                       "unstable"@en .


gtfs:locationType rdf:type owl:ObjectProperty ;
                  rdfs:domain gtfs:Location ;
                  rdfs:range [ owl:intersectionOf ( <http://www.w3.org/2004/02/skos/core#Concept>
                                                    [ rdf:type owl:Restriction ;
                                                      owl:onProperty <http://www.w3.org/2004/02/skos/core#inScheme> ;
                                                      owl:hasValue <http://transport.linkeddata.es/kos/location-type> ;
                                                    ]
                                                  ) ;
                                rdf:type owl:Class
                              ] ;
                  rdfs:comment "  Location type. 0 (or empty) - Stop. 1 - Station. 2 - Entrance/Exit. 3 - Generic Node. 4 - Boarding Area."@en ;
                  rdfs:label "LocationType"@en .


###  http://vocab.gtfs.org/terms#wheelchairAccessible
gtfs:wheelchairAccessible rdf:type owl:ObjectProperty ;
                          rdfs:domain [rdf:type owl:Class; 
                                       owl:unionOf (gtfs:Station
                                                    gtfs:Trip
                                                    gtfs:Stop
                                                   )
                                      ];
                          rdfs:range [ owl:intersectionOf ( <http://www.w3.org/2004/02/skos/core#Concept>
                                        [ rdf:type owl:Restriction ;
                                          owl:onProperty <http://www.w3.org/2004/02/skos/core#inScheme> ;
                                          owl:hasValue <http://transport.linkeddata.es/kos/wheelchair-accesible> ;
                                        ]
                                        ) ;
                                        rdf:type owl:Class
                                      ] ;
                          gtfs:comment "Si wheelchair_accessible es 0, mapee a gtfs:CheckParentStation; si es 1, mapee a gtfs:WheelchairAccessible; si es 2, mapee a gtfs:NotWheelchairAccessible."@es ,
                                       "When wheelchair_accessible is 0, map to gtfs:CheckParentStation; if 1 map to gtfs:WheelchairAccessible; if 2 map to gtfs:NotWheelchairAccessible."@en ;
                          rdfs:comment "La parada o estación específica es accesible para silla de ruedas. Si esta parada es parte de una estación, hay también una ruta accesible desde el exterior de la estación hasta la parada."@es ,
                                       "Wheelchair boardings are possible from the specified stop or station. If this stop is part of a station, there is also a wheelchair accessible path from outside the station towards the stop."@en ;
                          rdfs:label "accesible para silla de ruedas"@es ,
                                     "wheelchair boarding"@en ;
                          status:term_status "inestable"@es ,
                                             "unstable"@en .


###  http://vocab.gtfs.org/terms#timepoint
gtfs:timepoint rdf:type owl:ObjectProperty ;
               rdfs:domain gtfs:StopTime ;
               rdfs:range [ owl:intersectionOf ( <http://www.w3.org/2004/02/skos/core#Concept>
                                                  [ rdf:type owl:Restriction ;
                                                    owl:onProperty <http://www.w3.org/2004/02/skos/core#inScheme> ;
                                                    owl:hasValue <http://transport.linkeddata.es/kos/timepoint> ;
                                                  ]
                                                ) ;
                            rdf:type owl:Class
                          ] ;
               rdfs:comment "Indicates if arrival and departure times for a stop are strictly adhered to by the vehicle or if they are instead approximate and/or interpolated times. This field allows a GTFS producer to provide interpolated stop-times, while indicating that the times are approximate. [0 - Times are considered approximate, 1 or empty - Times are considered exact.]"@en ;
               rdfs:label "Timepoint"@en .


###  http://vocab.gtfs.org/terms#direction
gtfs:direction rdf:type owl:ObjectProperty ;
               rdfs:domain gtfs:Trip ;
               rdfs:range [ owl:intersectionOf ( <http://www.w3.org/2004/02/skos/core#Concept>
                                                         [ rdf:type owl:Restriction ;
                                                           owl:onProperty <http://www.w3.org/2004/02/skos/core#inScheme> ;
                                                           owl:hasValue <http://transport.linkeddata.es/kos/direction>;
                                                         ]
                                                       ) ;
                                    rdf:type owl:Class
                                  ] ;
               rdfs:comment "A binary property to indicate the direction the trip is going (outbound/inbound)"@en ,
                            "Apunta a un valor binario que indica la dirección del viaje (ida/vuelta)"@es ;
               rdfs:label "Direction"@en ,
                          "dirección"@es ;
               status:term_status "inestable"@es ,
                                  "unstable"@en .


###  http://vocab.gtfs.org/terms#bikesAllowed
gtfs:bikesAllowed rdf:type owl:ObjectProperty ;
                  rdfs:range [ owl:intersectionOf ( <http://www.w3.org/2004/02/skos/core#Concept>
                                                         [ rdf:type owl:Restriction ;
                                                           owl:onProperty <http://www.w3.org/2004/02/skos/core#inScheme> ;
                                                           owl:hasValue <http://transport.linkeddata.es/kos/bikes-allowed>;
                                                         ]
                                                       ) ;
                                    rdf:type owl:Class
                                  ] ;
                  rdfs:label "Bikes allowed"@en ,
                             "bicicletas permitidas"@es ;
                  status:term_status "inestable"@es ,
                                     "unstable"@en .


#################################################################
#    Data properties
#################################################################

#gtfs:Agency

gtfs:id rdf:type owl:DatatypeProperty ;
        rdfs:domain [ rdf:type owl:Class ;
                      owl:unionOf ( gtfs:Agency
                                    gtfs:Route
                                    gtfs:Shape
                                    gtfs:Service
                                    gtfs:Location
                                    gtfs:Trip
                                  )
                    ] ;
        rdfs:range dct:identifier ;
        rdfs:comment "Identifies a transit agency, a route, a shape, a set of dates when service is available, a location, a trip or a zone for a stop."@en ;
        rdfs:label "ID"@en .


gtfs:name rdf:type owl:DatatypeProperty ;
          rdfs:domain [rdf:type owl:Class ;
                       owl:unionOf (gtfs:Agency
                                    gtfs:Location
                                   )
                       ];
          rdfs:range foaf:name ;
          rdfs:comment "Full name of the transit agency or the location."@en ;
          rdfs:label "Name"@en .

 
gtfs:url rdf:type owl:DatatypeProperty ;
         rdfs:domain [rdf:type owl:Class ;
                      owl:unionOf (gtfs:Agency
                                   gtfs:Route
                                   gtfs:Location
                                   gtfs:Feed
                                  )
                      ];
         rdfs:range foaf:page ;
         rdfs:comment "URL of the transit agency, a particular route, a location, a publisher of a feed or a contact information URL."@en ;
         rdfs:label "URL"@en .


###  http://vocab.gtfs.org/terms#timezone
gtfs:timezone rdf:type owl:DatatypeProperty ;
              rdfs:domain [rdf:type owl:Class ; 
                           owl:unionOf (gtfs:Agency
                                        gtfs:Location
                                      )
                           ];
              rdfs:range xsd:string ;
              rdfs:comment "Timezone of the agency or the location."@en ;
              rdfs:label "Timezone"@en .


gtfs:language rdf:type owl:DatatypeProperty ;
              rdfs:domain [rdf:type owl:Class; 
                           owl:unionOf (gtfs:Agency
                                        gtfs:Feed
                                       )
                           ];
              rdfs:range dct:language ;
              rdfs:comment "Language used by a transit agency, used for the text in the GTFS dataset or default language used when the data consumer doesn’t know the language of the rider."@en ;
              rdfs:label "Language"@en .


gtfs:phoneNumber rdf:type owl:DatatypeProperty ;
                 rdfs:domain gtfs:Agency ;
                 rdfs:range foaf:phone ;
                 rdfs:comment "A voice telephone number for the specified agency."@en ;
                 rdfs:label "PhoneNumber"@en .


###  http://vocab.gtfs.org/terms#fareUrl
gtfs:fareUrl rdfs:comment "La URL de una página web que permite a un usuario comprar online billetes u otros productos de transporte de esa empresa"@es ,
                          "The URL of a web page that allows a rider to purchase tickets or other fare instruments for that agency online"@en ;
             rdfs:label "URL de tarifas"@es ,
                        "fare URL"@en ;
             rdfs:seeAlso <https://developers.google.com/transit/gtfs/reference#agency_fields> ;
             status:term_status "inestable"@es ,
                                "unstable"@en ;
             rdf:type owl:DatatypeProperty ;
             rdfs:range foaf:page ;
             rdfs:domain gtfs:Agency .


#gtfs:Route

###  http://vocab.gtfs.org/terms#longName
gtfs:longName rdfs:comment "Long name given to a route. This name is generally more descriptive than the gtfs:shortName and often includes the route's destination or stop."@en ,
                           "Nombre completo de una ruta"@es ;
              rdfs:label "Long name"@en ,
                         "nombre completo"@es ;
              rdfs:seeAlso <https://developers.google.com/transit/gtfs/examples/display-to-users#RouteLongName> ;
              status:term_status "inestable"@es ,
                                 "unstable"@en ;
              rdf:type owl:DatatypeProperty ;
              rdfs:range dct:title ;
              rdfs:domain gtfs:Route .


###  http://vocab.gtfs.org/terms#shortName
gtfs:shortName rdfs:comment "Nombre corto dado a una ruta o viaje"@es ,
                            "Short name given to a route or a trip"@en ;
               rdfs:label "Short name"@en ,
                          "nombre corto"@es ;
               rdfs:seeAlso <https://developers.google.com/transit/gtfs/examples/display-to-users#RouteShortName> ;
               status:term_status "inestable"@es ,
                                  "unstable"@en ;
               rdf:type owl:DatatypeProperty ;
               rdfs:range dct:title ;
               rdfs:domain [rdf:type owl:Class; 
                            owl:unionOf (gtfs:Route
                                         gtfs:Trip
                                        )
                           ].


gtfs:desc rdf:type owl:DatatypeProperty ;
          rdfs:domain [rdf:type owl:Class; 
                            owl:unionOf (gtfs:Route
                                         gtfs:Location
                                        )
                           ];
          rdfs:range dct:description ;
          rdfs:comment "Description of a route or a location that provides useful, quality information."@en ;
          rdfs:label "RouteDesc"@en .


###  http://vocab.gtfs.org/terms#color
gtfs:color rdf:type owl:DatatypeProperty ;
           rdfs:domain gtfs:Route ;
           rdfs:range xsd:string ;
           rdfs:comment "A 6 character hexidecimal color (without #) that matches the route color in public facing material"@en ,
                        "Un color expresado con 6 caracteres hexadecimales (sin #)"@es ;
           rdfs:label "Color"@en ,
                      "color"@es ;
           status:term_status "inestable"@es ,
                              "unstable"@en .


###  http://vocab.gtfs.org/terms#textColor
gtfs:textColor rdf:type owl:DatatypeProperty ;
               rdfs:domain gtfs:Route ;
               rdfs:range xsd:string ;
               rdfs:comment "A 6 character hexidecimal color (without #) asigned to a text label that is legible when written on top of a background of gtfs:color."@en ,
                            "Un color expresado con 6 caracteres hexadecimales (sin #) asignado a una etiqueta de texto."@es ;
               rdfs:label "Text color"@en ,
                          "color de texto"@es ;
               status:term_status "inestable"@es ,
                                  "unstable"@en .


###  http://vocab.gtfs.org/terms#sortOrder
gtfs:sortOrder rdf:type owl:DatatypeProperty ;
               rdfs:domain gtfs:Route ;
               rdfs:range xsd:nonNegativeInteger ;
               rdfs:comment "Orders the routes in a way which is ideal for presentation to customers."@en ;
               rdfs:label "Sort Order"@en .


#gtfs:Shape,gtfs:ShapePoint

gtfs:nonNegativeFloat a rdfs:Datatype ;
                        rdfs:subClassOf xsd:float ;
                        owl:onDatatype xsd:float ;
                        owl:withRestrictions (
                                                [ xsd:minInclusive "0.0"^^xsd:float ]
                                              ) .

###  http://vocab.gtfs.org/terms#distanceTraveled
gtfs:distanceTraveled rdf:type owl:DatatypeProperty ;
                      rdfs:domain [rdf:type owl:Class; 
                           owl:unionOf (gtfs:Shape
                                        gtfs:StopTime
                                       )
                           ];
                      rdfs:range gtfs:nonNegativeFloat ;
                      rdfs:comment "Indica la distancia a una parada desde el primer punto del recorrido. Representa una distancia de viaje real durante la ruta en unidades expresadas como pies o kilómetros. Esta información permite que quien planifica el viaje determine la porción de la forma que se debe trazar al mostrar parte de un viaje en el mapa. Los valores utilizados para gtfs:distanceTraveled se deben incrementar junto con los de gtfs:stopSequence, es decir, no se pueden usar para mostrar el recorrido inverso a lo largo de una ruta."@es ,
                                   "Positions a stop as a distance from the first shape point. It represents a real distance traveled along the route in units such as feet or kilometers. This information allows the trip planner to determine how much of the shape to draw when showing part of a trip on the map. The values used for gtfs:distanceTraveled must increase along with gtfs:stopSequence: they cannot be used to show reverse travel along a route."@en ;
                      rdfs:label "Distance Traveled"@en ,
                                 "distancia recorrida"@es ;
                      status:term_status "inestable"@es ,
                                         "unstable"@en .


gtfs:latitude rdf:type owl:DatatypeProperty ;
              rdfs:domain [rdf:type owl:Class; 
                           owl:unionOf (gtfs:ShapePoint
                                        gtfs:Stop
                                       )
                           ];
              rdfs:range geo:lat ;
              rdfs:comment "Latitude of a shape point or a stop."@en ;
              rdfs:label "Latitude"@en .


gtfs:longitude rdf:type owl:DatatypeProperty ;
               rdfs:domain [rdf:type owl:Class; 
                            owl:unionOf (gtfs:ShapePoint
                                         gtfs:Stop
                                        )
                           ];
               rdfs:range geo:long ;
               rdfs:comment "Longitude of a shape point or a stop."@en ;
               rdfs:label "Longitude"@en .


###  http://vocab.gtfs.org/terms#pointSequence
gtfs:pointSequence rdf:type owl:DatatypeProperty ;
                   rdfs:domain gtfs:ShapePoint ;
                   rdfs:range xsd:nonNegativeInteger ;
                   rdfs:comment "El campo gtfs:pointSequence asocia la latitud y longitud de un punto de recorrido con su orden de secuencia en el recorrido. Los valores para gtfs:pointSequence deben ser números enteros positivos y crecientes conforme avanza el viaje."@es ,
                                "The gtfs:pointSequence field associates the latitude and longitude of a shape point with its sequence order along the shape. The values for gtfs:pointSequence must be non-negative integers, and they must increase along the trip."@en ;
                   rdfs:label "Point Sequence"@en ,
                              "secuencia de puntos"@es ;
                   status:term_status "inestable"@es ,
                                      "unstable"@en .


#gtfs:Service,gtfs:ServiceRule,gtfs:CalendarRule,gtfs:CalendarDateRule

gtfs:startDate rdf:type owl:DatatypeProperty ;
               rdfs:domain [rdf:type owl:Class; 
                            owl:unionOf (gtfs:CalendarRule
                                         gtfs:Feed
                                        )
                           ];
               rdfs:range schema:startDate ;
               rdfs:comment "Start service day for the service interval or start date for which the GTFS data is valid."@en ;
               rdfs:label "StartDate"@en .


gtfs:endDate rdf:type owl:DatatypeProperty ;
             rdfs:domain [rdf:type owl:Class; 
                          owl:unionOf (gtfs:CalendarRule
                                       gtfs:Feed
                                      )
                           ];
             rdfs:range schema:endDate ;
             rdfs:comment "End service day for the service interval or end date for which the GTFS data is valid."@en ;
             rdfs:label "EndDate"@en .


gtfs:date rdf:type owl:DatatypeProperty ;
          rdfs:domain gtfs:CalendarDateRule ;
          rdfs:range dct:date ;
          rdfs:comment "Date when service exception occurs."@en ;
          rdfs:label "Date"@en .


#gtfs:Frequency 

###  http://vocab.gtfs.org/terms#startTime
gtfs:startTime rdf:type owl:DatatypeProperty ;
               rdfs:domain gtfs:Frequency ;
               rdfs:range schema:startTime ;
               rdfs:comment "Define la hora a la que empieza el servicio con la frecuencia especificada"@es ,
                            "Specifies the time at which service begins with the specified frequency"@en ;
               rdfs:label "Start Time"@en ,
                          "hora de inicio"@es ;
               status:term_status "inestable"@es ,
                                  "unstable"@en .


###  http://vocab.gtfs.org/terms#endTime
gtfs:endTime rdf:type owl:DatatypeProperty ;
             rdfs:domain gtfs:Frequency ;
             rdfs:range schema:endTime ;
             rdfs:comment "Define la hora a la que el servicio cambia de frecuencia (o bien finaliza) en la primera parada del viaje."@es ,
                          "Indicates the time at which service changes to a different frequency (or ceases) at the first stop in the trip."@en ;
             rdfs:label "End Time"@en ,
                        "hora final"@es ;
             status:term_status "inestable"@es ,
                                "unstable"@en .


###  http://vocab.gtfs.org/terms#headwaySeconds
gtfs:headwaySeconds rdf:type owl:DatatypeProperty ;
                    rdfs:domain gtfs:Frequency ;
                    rdfs:range xsd:positiveInteger ;
                    rdfs:comment "Indica el período de tiempo (en segundos) entre salidas desde la misma parada (tiempo entre viajes) para este tipo de viaje, durante el intervalo de tiempo especificado mediante start_time y end_time."@es ,
                                 "Indicates the time between departures from the same stop (headway) for this trip type, during the time interval specified by gtfs:startTime and gtfs:endTime."@en ;
                    rdfs:label "Headway Seconds"@en ,
                               "tiempo entre viajes"@es ;
                    status:term_status "inestable"@es ,
                                       "unstable"@en .


#gtfs:Location,gtfs:Stop,gtfs:Station

gtfs:code rdf:type owl:DatatypeProperty ;
          rdfs:domain gtfs:Location ;
          rdfs:range xsd:string ;
          status:term_status "unstable"@en ;
          rdfs:seeAlso <https://developers.google.com/transit/gtfs/reference#stops_fields> ;         
          rdfs:comment "Short text or a number that identifies the location for riders. These codes are often used in phone-based transit information systems or printed on signage to make it easier for riders to get information for a particular location. This field should be left empty for locations without a code presented to riders."@en ;
          rdfs:label "Location Code"@en .


#gtfs:StopTime

###  http://vocab.gtfs.org/terms#arrivalTime
gtfs:arrivalTime rdf:type owl:DatatypeProperty ;
                 rdfs:domain gtfs:StopTime ;
                 rdfs:range schema:Time ;
                 rdfs:comment "Check the original specification for special cases"@en ,
                              "Compruebe la especificación original para casos especiales"@es ;
                 rdfs:label "Arrival time"@en ,
                            "hora de llegada"@es ;
                 rdfs:seeAlso <https://developers.google.com/transit/gtfs/reference#stop_times_fields> ;
                 status:term_status "inestable"@es ,
                                    "unstable"@en .


###  http://vocab.gtfs.org/terms#departureTime
gtfs:departureTime rdf:type owl:DatatypeProperty ;
                   rdfs:domain gtfs:StopTime ;
                   rdfs:range schema:Time ;
                   rdfs:comment "Check the original specification for special cases"@en ,
                                "Compruebe la especificación original para casos especiales"@es ;
                   rdfs:label "Departure time"@en ,
                              "hora de salida"@es ;
                   rdfs:seeAlso <https://developers.google.com/transit/gtfs/reference#stop_times_fields> ;
                   status:term_status "inestable"@es ,
                                      "unstable"@en .


###  http://vocab.gtfs.org/terms#stopSequence
gtfs:stopSequence rdf:type owl:DatatypeProperty ;
                  rdfs:domain gtfs:StopTime ;
                  rdfs:range xsd:nonNegativeInteger ;
                  rdfs:comment "Indica el orden de paradas para un viaje concreto. Los valores de gtfs:stopSequence deben ser enteros no negativos, deben aumentar durante el viaje referenciado por la propiedad gtfs:trip."@es ,
                               "The stopSequence property identifies the order of the stops for a particular trip. The values must increase along the gtfs:Trip referenced in the gtfs:trip property."@en ;
                  rdfs:label "Stop sequence"@en ,
                             "secuencia de paradas"@es ;
                  status:term_status "inestable"@es ,
                                     "unstable"@en .


###  http://vocab.gtfs.org/terms#headsign
gtfs:headsign rdf:type owl:DatatypeProperty ;
              rdfs:domain [rdf:type owl:Class; 
                           owl:unionOf (gtfs:StopTime
                                        gtfs:Trip
                                       )
                           ];
              rdfs:range xsd:string ;
              rdfs:comment "Esta propiedad apunta al texto que indica el destino del viaje a los pasajeros."@es ,
                           "The gtfs:headsign property contains the text that appears on a sign that identifies the trip's destination to passengers."@en ;
              rdfs:label "Headsign"@en ,
                         "destino del viaje"@es ;
              rdfs:seeAlso <https://developers.google.com/transit/gtfs/examples/display-to-users#TripHeadsign> ;
              status:term_status "inestable"@es ,
                                 "unstable"@en .


#gtfs:Trip

###  http://vocab.gtfs.org/terms#block
gtfs:block rdf:type owl:DatatypeProperty ;
           rdfs:domain gtfs:Trip ;
           rdfs:range dct:identifier;
           rdfs:comment "Identifies the block to which the trip within this feed belongs. A block consists of two or more sequential trips made using the same vehicle, where a passenger can transfer from one trip to the next just by staying in the vehicle."@en ,
                        "Identifica el bloque al que pertenece el viaje. Un bloque consta de dos o más viajes secuenciales realizados en el mismo vehículo, en los que un pasajero puede cambiar de viaje si simplemente permanece en el vehículo."@es ;
           rdfs:label "Block"@en ,
                      "Bloque"@es ;
           status:term_status "unstable"@en ,
                              "inestable"@es .


#gtfs:Feed

gtfs:publisher rdf:type owl:DatatypeProperty ;
               rdfs:domain gtfs:Feed ;
               rdfs:range dct:publisher ;
               rdfs:comment "Full name of the organization that publishes the dataset."@en ;
               rdfs:label "Publisher"@en .


gtfs:version rdf:type owl:DatatypeProperty ;
             rdfs:domain gtfs:Feed ;
             rdfs:range schema:version ;
             rdfs:comment "String that indicates the current version of their GTFS dataset."@en ;
             rdfs:label "Version"@en .

      
###  http://vocab.gtfs.org/terms#bidirectional
gtfs:bidirectional rdf:type owl:DatatypeProperty ;
                   rdfs:domain gtfs:Pathway ;
                   rdfs:range xsd:boolean ;
                   rdfs:comment "Indicates in which direction the pathway can be used: [0: Unidirectional pathway, it can only be used from gtfs:originStop to gtfs:destinationStop,  1: Bidirectional pathway, it can be used in the two directions]"@en ;
                   rdfs:label "Index"@en .


###  http://vocab.gtfs.org/terms#index
gtfs:index rdf:type owl:DatatypeProperty ;
           rdfs:domain gtfs:Level ;
           rdfs:range xsd:float ;
           rdfs:comment "Numeric index of the level that indicates relative position of this level in relation to other levels (levels with higher indices are assumed to be located above levels with lower indices). Ground level should have index 0, with levels above ground indicated by positive indices and levels below ground by negative indices."@en ;
           rdfs:label "Index"@en .


###  http://vocab.gtfs.org/terms#isAuthority
gtfs:isAuthority rdf:type owl:DatatypeProperty ;
                 rdfs:domain gtfs:Attribution ;
                 rdfs:range xsd:boolean ;
                 rdfs:comment "A binary value indicating whether the role of the organization is authority. Allowed values include the following: [0 or empty: Organization doesn’t have this role, 1: Organization does have this role.]"@en ;
                 rdfs:label "Is Authority?"@en .


###  http://vocab.gtfs.org/terms#isOperator
gtfs:isOperator rdf:type owl:DatatypeProperty ;
                rdfs:domain gtfs:Attribution ;
                rdfs:range xsd:boolean ;
                rdfs:comment "A binary value indicating whether the role of the organization is operator. Allowed values include the following: [0 or empty: Organization doesn’t have this role, 1: Organization does have this role.]"@en ;
                rdfs:label "Is Operator?"@en .


###  http://vocab.gtfs.org/terms#isProducer
gtfs:isProducer rdf:type owl:DatatypeProperty ;
                rdfs:domain gtfs:Attribution ;
                rdfs:range xsd:boolean ;
                rdfs:comment "A binary value indicating whether the role of the organization is producer. Allowed values include the following: [0 or empty: Organization doesn’t have this role, 1: Organization does have this role.]"@en ;
                rdfs:label "Is Producer?"@en .


###  http://vocab.gtfs.org/terms#length
gtfs:length rdf:type owl:DatatypeProperty ;
            rdfs:domain gtfs:Pathway ;
            rdfs:range xsd:float ;
            rdfs:comment "Horizontal length in meters of the pathway from the origin location (defined in from_stop_id) to the destination location (defined in to_stop_id)."@en ;
            rdfs:label "Length"@en .


###  http://vocab.gtfs.org/terms#maxSlope
gtfs:maxSlope rdf:type owl:DatatypeProperty ;
              rdfs:domain gtfs:Pathway ;
              rdfs:range xsd:float ;
              rdfs:comment "Maximum slope ratio of the pathway. Valid values for this field are:[ 0 or (empty): no slope, A float: slope ratio of the pathway, positive for upwards, negative for downwards.]"@en ;
              rdfs:label "Max Slope"@en .


###  http://vocab.gtfs.org/terms#minWidth
gtfs:minWidth rdf:type owl:DatatypeProperty ;
              rdfs:domain gtfs:Pathway ;
              rdfs:range xsd:float ;
              rdfs:comment "Minimum width of the pathway in meters. This field is highly recommended if the minimum width is less than 1 meter."@en ;
              rdfs:label "Min Width"@en .


###  http://vocab.gtfs.org/terms#minimumTransferTime
gtfs:minimumTransferTime rdf:type owl:DatatypeProperty ;
                         rdfs:domain gtfs:TransferRule ;
                         rdfs:range xsd:nonNegativeInteger ;
                         rdfs:comment "El tiempo mínimo de transbordo cuando gtfs:transferType es gtfs:MinimumTimeTransfer."@es ,
                                      "The minimum transfer time when the gtfs:transferType is gtfs:MinimumTimeTransfer. It is an amount of time, in seconds, that must be available to permit a transfer between routes at the specified stops. It should be sufficient to permit a typical rider to move between the two stops, including buffer time to allow for schedule variance on each route."@en ;
                         rdfs:label "Minimum Transfer Time"@en ,
                                    "Tiempo mínimo de transbordo"@es ;
                         status:term_status "inestable"@es ,
                                            "unstable"@en .


###  http://vocab.gtfs.org/terms#platformCode
gtfs:platformCode rdf:type owl:DatatypeProperty ;
                  rdfs:domain gtfs:Platform ;
                  rdfs:range xsd:string ;
                  rdfs:comment "Platform identifier for a platform stop (a stop belonging to a station). This should be just the platform identifier (eg. G or 3). Words like platform or track (or the feed’s language-specific equivalent) should not be included. This allows feed consumers to more easily internationalize and localize the platform identifier into other languages."@en ;
                  rdfs:label "Platform Code"@en .


###  http://vocab.gtfs.org/terms#reversedSignpostedAs
gtfs:reversedSignpostedAs rdf:type owl:DatatypeProperty ;
                          rdfs:domain gtfs:Pathway ;
                          rdfs:range xsd:string ;
                          rdfs:comment "Same as the gtfs:signpostedAs but when the pathways is used backward, i.e. from the gtfs:destinationStop to the gtfs:originStop."@en ;
                          rdfs:label "Reversed Signposted As"@en .


###  http://vocab.gtfs.org/terms#signpostedAs
gtfs:signpostedAs rdf:type owl:DatatypeProperty ;
                  rdfs:domain gtfs:Pathway ;
                  rdfs:range xsd:string ;
                  rdfs:comment "String of text from physical signage visible to transit riders. The string can be used to provide text directions to users, such as 'follow signs to '. The language text should appear in this field exactly how it is printed on the signs - it should not be translated."@en ;
                  rdfs:label "Signposted As"@en .


###  http://vocab.gtfs.org/terms#stairCount
gtfs:stairCount rdf:type owl:DatatypeProperty ;
                rdfs:domain gtfs:Pathway ;
                rdfs:range xsd:integer ;
                rdfs:comment "Number of stairs of the pathway. Best Practices: one could use the approximation of 1 floor = 15 stairs to generate approximative values."@en ;
                rdfs:label "Stair Count"@en .


###  http://vocab.gtfs.org/terms#transferDuration
gtfs:transferDuration rdf:type owl:DatatypeProperty ;
                      rdfs:domain gtfs:FareClass ;
                      rdfs:range xsd:nonNegativeInteger ;
                      rdfs:comment "Length of time in seconds before a transfer expires. When transfers=0 this field can be used to indicate how long a ticket is valid for or it can can be left empty."@en ;
                      rdfs:label "Transfer Duration"@en .


###  http://vocab.gtfs.org/terms#traversalTime
gtfs:traversalTime rdf:type owl:DatatypeProperty ;
                   rdfs:domain gtfs:Pathway ;
                   rdfs:range xsd:positiveInteger ;
                   rdfs:comment "Average time in seconds needed to walk through the pathway from the gtfs:originStop to the gtfs:destinationStop."@en ;
                   rdfs:label "Traversal Time"@en .


#################################################################
#    Classes
#################################################################

###  http://schema.org/PriceSpecification
schema:PriceSpecification rdf:type owl:Class .


###  http://vocab.gtfs.org/terms#Agency
gtfs:Agency rdf:type owl:Class ;
            rdfs:subClassOf foaf:Agent ;
            rdfs:comment "An agency operates a certain schedule based transport mode"@en ,
                         "Una empresa opera un cierto modo de transporte de manera programada"@es ;
            rdfs:label "Agency"@en ,
                       "Empresa"@es ;
            rdfs:seeAlso <https://developers.google.com/transit/gtfs/reference#agency_fields> ;
            status:term_status "estable"@es ,
                               "stable"@en .


###  http://vocab.gtfs.org/terms#Attribution
gtfs:Attribution rdf:type owl:Class ;
                 rdfs:comment "Identifies an attribution for the dataset, or a subset of it. This field is useful for translations."@en ;
                 rdfs:label "Attribution"@en .


###  http://vocab.gtfs.org/terms#Block
gtfs:Block rdf:type owl:Class ;
           rdfs:comment "A block consists of a single trip or many sequential trips made using the same vehicle, defined by shared service days and block ID."@en ;
           rdfs:label "Block"@en .


###  http://vocab.gtfs.org/terms#BoardingArea
gtfs:BoardingArea rdf:type owl:Class ;
                  rdfs:subClassOf gtfs:Location ;
                  rdfs:comment "A specific location on a platform, where passengers can board and/or alight vehicles."@en ;
                  rdfs:label "Boarding Area"@en .


###  http://vocab.gtfs.org/terms#CalendarRule
gtfs:CalendarRule rdf:type owl:Class ;
                  rdfs:subClassOf gtfs:ServiceRule ;
                  gtfs:comment "a row from calendar.txt"@en ,
                               "una línea de calendar.txt"@es ;
                  rdfs:comment "Defines on which days of the week for a certain period the service is available."@en ,
                               "Define en qué días de la semana el servicio está disponible para un periodo concreto."@es ;
                  rdfs:label "Calendar rule"@en ,
                             "Regla de calendario"@es ;
                  status:term_status "inestable"@es ,
                                     "unstable"@en .


###  http://vocab.gtfs.org/terms#CalendarDateRule
gtfs:CalendarDateRule rdf:type owl:Class ;
                      gtfs:comment "a row from calendar_dates.txt"@en ,
                                   "una línea en calendar_dates.txt"@es ;
                      rdfs:comment "Defines exceptions for the services defined in gtfs:Service."@en ,
                                   "Indica la disponibilidad de servicio para una fecha concreta"@es ;
                      rdfs:label "Calendar date rule"@en ,
                                 "Regla de fecha de calendario"@es ;
                      rdfs:seeAlso <https://developers.google.com/transit/gtfs/reference#calendar_dates_fields> ;
                      status:term_status "inestable"@es ,
                                         "unstable"@en .


###  http://vocab.gtfs.org/terms#ContinuousDropOff
gtfs:ContinuousDropOff rdf:type owl:Class ;
                       rdfs:subClassOf gtfs:DropOffType ;
                       rdfs:comment "A type of drop off where a rider can alight the vehicle anywhere along the vehicle's travel path."@en ;
                       rdfs:label "Continuous Drop Off"@en .


###  http://vocab.gtfs.org/terms#ContinuousPickup
gtfs:ContinuousPickup rdf:type owl:Class ;
                      rdfs:subClassOf gtfs:PickupType ;
                      rdfs:comment "A type of pickup where a rider can board the transit vehicle anywhere along the vehicle’s travel path."@en ;
                      rdfs:label "Continuous Pickup"@en .


###  http://vocab.gtfs.org/terms#DropOffType
gtfs:DropOffType rdf:type owl:Class ;
                 rdfs:comment "Instances of this class can be used by gtfs:dropOffType"@en ,
                              "Instancias de esta clase pueden ser usadas por gtfs:dropOffType. Indica si los pasajeros se bajan en una parada como parte del horario normal o si no pueden bajar en esa parada."@es ;
                 rdfs:label "Drop Off Type"@en ,
                            "Tipo de bajada"@es ;
                 status:term_status "inestable"@es ,
                                    "unstable"@en .


###  http://vocab.gtfs.org/terms#Elevator
gtfs:Elevator rdf:type owl:Class .


###  http://vocab.gtfs.org/terms#Escalator
gtfs:Escalator rdf:type owl:Class .


###  http://vocab.gtfs.org/terms#ExitGate
gtfs:ExitGate rdf:type owl:Class .


###  http://vocab.gtfs.org/terms#FareClass
gtfs:FareClass rdf:type owl:Class ;
               rdfs:subClassOf schema:PriceSpecification ;
               gtfs:comment "A gtfs:FareClass corresponds to a row in the fare_attributes.txt file."@en ,
                            "Una gtfs:FareClass corresponde a una línea en fare_attributes.txt."@es ;
               rdfs:comment "A class describing how the fare is calculated."@en ,
                            "Describe como se calcula la tarifa."@es ;
               rdfs:label "Clase tarifaria"@es ,
                          "Fare Class"@en ;
               rdfs:seeAlso <https://code.google.com/p/googletransitdatafeed/wiki/FareExamples> ,
                            <https://developers.google.com/transit/gtfs/reference#fare_attributes_fields> ,
                            <https://developers.google.com/transit/gtfs/reference#fare_rules_fields> ;
               status:term_status "inestable"@es ,
                                  "unstable"@en .


###  http://vocab.gtfs.org/terms#FareGate
gtfs:FareGate rdf:type owl:Class .


###  http://vocab.gtfs.org/terms#FareRule
gtfs:FareRule rdf:type owl:Class ;
              rdfs:comment "A rule which binds a gtfs:FareClass to a part of the network."@en ,
                           "Una regla que enlaza una clase tarifaria (gtfs:FareClass) a un zona de la red de transporte."@es ;
              rdfs:label "Fare Rule"@en ,
                         "Regla tarifaria"@es ;
              status:term_status "inestable"@es ,
                                 "unstable"@en .


###  http://vocab.gtfs.org/terms#Feed
gtfs:Feed rdf:type owl:Class ;
          rdfs:subClassOf dcat:Dataset ;
          rdfs:comment "An instance of a gtfs:Feed is a linked GTFS feed that complies to this specification."@en ,
                       "Una instancia de gtfs:Feed es un feed GTFS enlazado que cumple con esta especificación."@es ;
          rdfs:label "GTFS Feed"@en ,
                     "GTFS Feed"@es ;
          rdfs:seeAlso <https://developers.google.com/transit/gtfs/reference#feed_info_fields> ;
          status:term_status "estable"@es ,
                             "stable"@en ;
          dcat:theme <http://eurovoc.europa.eu/2015> .


###  http://vocab.gtfs.org/terms#Frequency
gtfs:Frequency rdf:type owl:Class ;
               rdfs:comment "An alternative to defining departures and arrivals as StopTimes: define frequencies for transit vehicle"@en ,
                            "Una alternativa a definir salidas y llegadas como StopTimes: definir frecuencias para vehículos de transporte público"@es ;
               rdfs:label "Frecuencia"@es ,
                          "Frequency"@en ;
               rdfs:seeAlso <https://developers.google.com/transit/gtfs/reference#frequencies_fields> ;
               status:term_status "inestable"@es ,
                                  "unstable"@en .


###  http://vocab.gtfs.org/terms#GenericNode
gtfs:GenericNode rdf:type owl:Class ;
                 rdfs:subClassOf gtfs:Location ;
                 rdfs:comment "A location within a station, not matching any other location type, which can be used to link together pathways."@en ;
                 rdfs:label "Generic Node"@en .


###  http://vocab.gtfs.org/terms#Level
gtfs:Level rdf:type owl:Class ;
           rdfs:comment "Describes the different levels (e.g. Mezzanine” or the “Platform” level) of a station. Is mostly useful when used in conjunction with gtfs:Pathway."@en ;
           rdfs:label "Level"@en .


###  http://vocab.gtfs.org/terms#Location
gtfs:Location rdf:type owl:Class ;
              rdfs:comment "A location is a geographical point that has a latitude and a longitude."@en ;
              rdfs:label "Location"@en .


###  http://vocab.gtfs.org/terms#MovingSidewalk
gtfs:MovingSidewalk rdf:type owl:Class .


###  http://vocab.gtfs.org/terms#Pathway
gtfs:Pathway rdf:type owl:Class ;
             rdfs:comment "A pathway links together locations within stations."@en ;
             rdfs:label "Pathway"@en .


###  http://vocab.gtfs.org/terms#PaymentMethod
gtfs:PaymentMethod rdf:type owl:Class ;
                   rdfs:comment "Method to pay for the public transit service"@en ,
                                "Método de pago para el servicio de transporte público"@es ;
                   rdfs:label "Método de pago"@es ,
                              "Payment Method"@en ;
                   status:term_status "inestable"@es ,
                                      "unstable"@en .


###  http://vocab.gtfs.org/terms#PickupType
gtfs:PickupType rdf:type owl:Class ;
                rdfs:comment "Instances of this class can be used by gtfs:pickupType"@en ,
                             "Instancias de esta clase pueden ser usadas por gtfs:pickupType. Indica si se recogen los pasajeros en una parada como parte del horario normal o si su recogida en dicha parada no se encuentra disponible. Este campo también permite a la empresa de transporte público indicar que los pasajeros deben llamar a la empresa o notificar al conductor que es necesario recogerlos en esa parada en concreto. Los valores válidos para este campo son: 0 - recogida programada regularmente; 1 - recogida no disponible; 2 - se debe llamar a la empresa para organizar una recogida; 3 - se debe coordinar con el conductor para organizar una recogida. El valor predeterminado de este campo es 0."@es ;
                rdfs:label "Pickup Type"@en ,
                           "Tipo de recogida"@es ;
                status:term_status "inestable"@es ,
                                   "unstable"@en .


###  http://vocab.gtfs.org/terms#Platform
gtfs:Platform rdf:type owl:Class ;
              rdfs:subClassOf gtfs:Location ;
              rdfs:comment "A stop existing inside a station."@en ;
              rdfs:label "Platform"@en .


###  http://vocab.gtfs.org/terms#Route
gtfs:Route rdf:type owl:Class ;
           rdfs:comment "A gtfs:Route is a commercial route followed entirely or partly by gtfs:Trips"@en ,
                        "Una gtfs:Route es un grupo de viajes (gtfs:Trips) que se muestran a los usuarios como servicio independiente"@es ;
           rdfs:label "Route"@en ,
                      "Ruta"@es ;
           rdfs:seeAlso <https://developers.google.com/transit/gtfs/reference#routes_fields> ;
           status:term_status "inestable"@es ,
                              "unstable"@en .


###  http://vocab.gtfs.org/terms#RouteType
gtfs:RouteType rdf:type owl:Class ;
               rdfs:domain gtfs:Route ;
               rdfs:comment "Describe el tipo de transporte usado en una ruta"@es ,
                            "Describes the type of transportation used on a route"@en ;
               rdfs:label "Route type"@en ,
                          "Tipo de ruta"@es ;
               status:term_status "inestable"@es ,
                                  "unstable"@en .


###  http://vocab.gtfs.org/terms#Service
gtfs:Service rdf:type owl:Class ;
             gtfs:comment "A gtfs:Service is a set of gtfs:ServiceRules which can be found in both calendar.txt as calendar_dates.txt"@en ,
                          "Un gtfs:Service es un conjunto de gtfs:ServiceRules que pueden ser encontradas en calendar.txt y calendar_dates.txt"@es ;
             rdfs:comment "Service dates specified using a weekly schedule with start and end dates."@en ,
                          "Un gtfs:Service indica el conjunto de fechas en el que el servicio está disponible para una o más rutas"@es ;
             rdfs:label "Service"@en ,
                        "Servicio"@es ;
             rdfs:seeAlso <https://developers.google.com/transit/gtfs/reference#calendar_dates_fields> ,
                          <https://developers.google.com/transit/gtfs/reference#calendar_fields> ;
             status:term_status "inestable"@es ,
                                "unstable"@en .


###  http://vocab.gtfs.org/terms#ServiceRule
gtfs:ServiceRule rdf:type owl:Class ;
                 rdfs:comment "One or more service rules define a set of dates"@en ,
                              "Una o más reglas de servicio definen un conjunto de fechas"@es ;
                 rdfs:label "Service rule"@en ,
                            "Regla de servicio"@es ;
                 status:term_status "unstable"@en ,
                                    "inestable"@es .                                


###  http://vocab.gtfs.org/terms#Shape
gtfs:Shape rdf:type owl:Class ;
           rdfs:comment "A polygon formed by gtfs:ShapePoints"@en ,
                        "Un polígono o línea formado por gtfs:ShapePoints"@es ;
           rdfs:label "Shape"@en ,
                      "forma del recorrido, trayecto, itinerario"@es ;
           rdfs:seeAlso <https://developers.google.com/transit/gtfs/reference#shapes_fields> ;
           status:term_status "inestable"@es ,
                              "unstable"@en .


###  http://vocab.gtfs.org/terms#ShapePoint
gtfs:ShapePoint rdf:type owl:Class ;
                rdfs:comment "A geographic point within a gtfs:Shape"@en ,
                             "Punto geográfico dentro de un recorrido (gtfs:Shape)"@es ;
                rdfs:label "Punto de recorrido"@es ,
                           "Shape Point"@en ;
                rdfs:seeAlso <https://developers.google.com/transit/gtfs/reference#shapes_fields> ;
                status:term_status "inestable"@es ,
                                   "unstable"@en .


###  http://vocab.gtfs.org/terms#SingleDropOff
gtfs:SingleDropOff rdf:type owl:Class ;
                   rdfs:subClassOf gtfs:DropOffType ;
                   rdfs:label "Single Drop Off"@en .


###  http://vocab.gtfs.org/terms#SinglePickup
gtfs:SinglePickup rdf:type owl:Class ;
                  rdfs:subClassOf gtfs:PickupType ;
                  rdfs:label "Single Pickup"@en .


###  http://vocab.gtfs.org/terms#Stairs
gtfs:Stairs rdf:type owl:Class .


###  http://vocab.gtfs.org/terms#Station
gtfs:Station rdf:type owl:Class ;
             rdfs:subClassOf gtfs:Location ;
             gtfs:comment "Map a row in stops.txt to gtfs:Station when the location_type is 1."@en ,
                          "Mapee una línea en stops.txt a gtfs:Station cuando location_type sea 1."@es ;
             rdfs:comment "A physical structure or area that contains one or more platform."@en ,
                          "Estructura física o área que contiene una o más paradas."@es ;
             rdfs:label "Estación"@es ,
                        "Station"@en ;
             rdfs:seeAlso <https://developers.google.com/transit/gtfs/reference#stops_fields> ;
             status:term_status "inestable"@es ,
                                "unstable"@en .


###  http://vocab.gtfs.org/terms#StationEntrance
gtfs:StationEntrance rdf:type owl:Class ;
                     rdfs:subClassOf gtfs:Location ;
                     rdfs:comment "A location where passengers can enter or exit a station from the street. If an entrance/exit belongs to multiple stations, it can be linked by pathways to both, but the data provider must pick one of them as parent."@en ;
                     rdfs:label "Station Entrance"@en .


###  http://vocab.gtfs.org/terms#Stop
gtfs:Stop rdf:type owl:Class ;
          rdfs:subClassOf gtfs:Location ;
          rdfs:comment "A stop is a physical location where a vehicle stops or leaves. Multiple routes may use the same stop."@en ,
                       "Un lugar donde los pasajeros suben o bajan de un vehículo de transporte público."@es ;
          rdfs:label "Parada"@es ,
                     "Stop"@en ;
          rdfs:seeAlso <https://developers.google.com/transit/gtfs/reference#stops_fields> ;
          status:term_status "estable"@es ,
                             "stable"@en .


###  http://vocab.gtfs.org/terms#StopTime
gtfs:StopTime rdf:type owl:Class ;
              rdfs:comment "Describe una hora de parada como parte de un viaje"@es ,
                           "Describes a stop time as part of a trip"@en ;
              rdfs:label "Hora de parada"@es ,
                         "Stop time"@en ;
              rdfs:seeAlso <https://developers.google.com/transit/gtfs/reference#stop_times_fields> ;
              status:term_status "inestable"@es ,
                                 "unstable"@en .


###  http://vocab.gtfs.org/terms#Transfer
gtfs:Transfer rdf:type owl:Class .


###  http://vocab.gtfs.org/terms#TransferRule
gtfs:TransferRule rdf:type owl:Class ;
                  rdfs:comment "Define additional rules for making connections between routes."@en ,
                               "Define reglas adicionales para transbordos entre rutas."@es ;
                  rdfs:label "Regla de transbordo"@es ,
                             "Transfer Rule"@en ;
                  rdfs:seeAlso <https://developers.google.com/transit/gtfs/reference#transfers_fields> ;
                  status:term_status "inestable"@es ,
                                     "unstable"@en .


###  http://vocab.gtfs.org/terms#TransferType
gtfs:TransferType rdf:type owl:Class ;
                  gtfs:comment "Si transfer_type en transfers.txt es 0 o vacío, mapee a gtfs:RecommendedTransfer; si es 1, mapee to gtfs:EnsuredTransfer; si es 2, a gtfs:MinimumTimeTransfer; si es 3, a gtfs:NoTransfer"@es ,
                               "When transfer_type in transfers.txt is 0 or empty, map to gtfs:RecommendedTransfer, when 1, map to gtfs:EnsuredTransfer, when 2, gtfs:MinimumTimeTransfer, when 3: gtfs:NoTransfer."@en ;
                  rdfs:comment "Instances of this class can be used to describe how to handle a transfer rule"@en ,
                               "Instancias de esta clase pueden ser usadas para describir cómo gestionar las reglas de transbordo"@es ;
                  rdfs:label "Tipo de transbordo"@es ,
                             "Transfer Type"@en ;
                  status:term_status "inestable"@es ,
                                     "unstable"@en .


###  http://vocab.gtfs.org/terms#TransfersAllowedType
gtfs:TransfersAllowedType rdf:type owl:Class ;
                          rdfs:comment "Instances of this class describe whether tickets remain valid when transferring"@en ,
                                       "Las instancias de esta clase describen si los billetes son válidos para realizar transbordos"@es ;
                          rdfs:label "Tipo de transbordo permitido"@es ,
                                     "Transfers Allowed Type"@en ;
                          status:term_status "inestable"@es ,
                                             "unstable"@en .


###  http://vocab.gtfs.org/terms#Translation
gtfs:Translation rdf:type owl:Class ;
                 rdfs:comment "Translated information of a transit agency."@en ;
                 rdfs:label "Translation"@en .


###  http://vocab.gtfs.org/terms#Trip
gtfs:Trip rdf:type owl:Class ;
          rdfs:comment "A collection of gtfs:StopTimes followed by a transit vehicle"@en ,
                       "Trayecto de dos o más paradas realizadas por un vehículo que se produce a una gtfs:StopTime"@es ;
          rdfs:label "Trip"@en ,
                     "Viaje"@es ;
          rdfs:seeAlso <https://developers.google.com/transit/gtfs/reference#trips_fields> ;
          status:term_status "inestable"@es ,
                             "unstable"@en .


###  http://vocab.gtfs.org/terms#Walkway
gtfs:Walkway rdf:type owl:Class .


###  http://vocab.gtfs.org/terms#WheelchairBoardingStatus
gtfs:WheelchairBoardingStatus rdf:type owl:Class ;
                              rdfs:comment "A class whom's instances indicate how accessible a gtfs:Trip, gtfs:Stop or gtfs:Station is."@en ,
                                           "Las instancias de esta clase indican como de accesible es un gtfs:Trip, un gtfs:Stop o una gtfs:Station."@es ;
                              rdfs:label "Información de accesibilidad para silla de ruedas"@es ,
                                         "Wheelchair Boarding Information"@en ;
                              rdfs:seeAlso <https://developers.google.com/transit/gtfs/reference#stops_fields> ;
                              status:term_status "inestable"@es ,
                                                 "unstable"@en .


###  http://vocab.gtfs.org/terms#Zone
gtfs:Zone rdf:type owl:Class ;
          rdfs:subClassOf gtfs:Location ;
          rdfs:comment "Las zonas son necesarias si quiere proporcionar información de tarifas usando gtfs:FareClass"@es ,
                       "Zones are required if you want to provide fare information using gtfs:FareClass. It is a space within a stop for which a specific fare applies."@en ;
          rdfs:label "Zona"@es ,
                     "Zone"@en ;
          status:term_status "inestable"@es ,
                             "unstable"@en .


###  http://www.w3.org/ns/dcat#Dataset
dcat:Dataset rdf:type owl:Class .


###  http://xmlns.com/foaf/0.1/Agent
foaf:Agent rdf:type owl:Class .


###  http://xmlns.com/foaf/0.1/Document
foaf:Document rdf:type owl:Class .


#################################################################
#    Individuals
#################################################################

###  http://vocab.gtfs.org/terms
<http://vocab.gtfs.org/terms> rdf:type owl:NamedIndividual ,
                                       foaf:Document ;
                              cc:license <http://creativecommons.org/licenses/by/3.0/> ;
                              dct:hasFormat <https://raw.githubusercontent.com/OpenTransport/vocabulary/master/gtfs/gtfs.ttl> ;
                              dct:issued "2014-10-23"^^xsd:date ;
                              dct:modified "2014-10-27"^^xsd:date ;
                              dct:rights "Copyright 2014 - Open Transport contributors" ;
                              foaf:primaryTopic <http://vocab.gtfs.org/terms#> .


###  http://vocab.gtfs.org/terms#BeforeBoarding
gtfs:BeforeBoarding rdf:type owl:NamedIndividual ,
                             gtfs:PaymentMethod ;
                    rdfs:comment "La tarifa se debe pagar antes de subir a bordo"@es ,
                                 "Ticket should be bought before boarding"@en ;
                    rdfs:label "Antes de subir a bordo"@es ,
                               "Before Boarding"@en ;
                    status:term_status "inestable"@es ,
                                       "unstable"@en .


###  http://vocab.gtfs.org/terms#Bus
gtfs:Bus rdf:type owl:NamedIndividual ,
                  gtfs:RouteType ;
         rdfs:comment "Used for short- and long-distance bus routes."@en ,
                      "Utilizado para rutas en autobús de corta y larga distancia."@es ;
         rdfs:label "Autobús"@es ,
                    "Bus"@en ;
         status:term_status "inestable"@es ,
                            "unstable"@en .


###  http://vocab.gtfs.org/terms#CableCar
gtfs:CableCar rdf:type owl:NamedIndividual ,
                       gtfs:RouteType ;
              rdfs:comment "Cable transport where cabins, cars, gondolas or open chairs are suspended by means of one or more cables."@en ,
                           "Normalmente se utiliza para medios de transporte público por cable en donde el vehículo queda suspendido de un cable."@es ;
              rdfs:label "Aerial lift, suspended cable car (e.g., gondola lift, aerial tramway)"@en ,
                         "Teleférico, telecabina"@es ;
              status:term_status "inestable"@es ,
                                 "unstable"@en ;
              adms:versionNotes "The definition of Gondola has been changed in the gtfs spec to now describe CableCar. CableCar is the new term for instances previously linked to Gondola." .


###  http://vocab.gtfs.org/terms#CableTram
gtfs:CableTram rdf:type owl:NamedIndividual ,
                        gtfs:RouteType ;
               rdfs:comment "Used for street-level rail cars where the cable runs beneath the vehicle."@en ,
                            "Utilizado para funiculares en superficie en donde el cable pasa por debajo del vehículo."@es ;
               rdfs:label "Cable Tram"@en ,
                          "Funicular"@es ;
               status:term_status "inestable"@es ,
                                  "unstable"@en ;
               adms:versionNotes "The definition of CableCar has been changed in the gtfs spec to now describe CableTram. CableTram is the new term for instances previously linked to CableCar." .


###  http://vocab.gtfs.org/terms#CheckParentStation
gtfs:CheckParentStation rdf:type owl:NamedIndividual ,
                                 gtfs:WheelchairBoardingStatus ;
                        gtfs:comment "Corresponde a wheelchair_accessible con valor 0."@es ,
                                     "Corresponds with wheelchair_accessible being 0."@en ;
                        rdfs:comment "Check the (parent) station for accessibility information."@en ,
                                     "Compruebe la estación (matriz) para información de accesibilidad."@es ;
                        rdfs:label "Check the parent station"@en ,
                                   "Compruebe la estación matriz"@es ;
                        status:term_status "inestable"@es ,
                                           "unstable"@en .


###  http://vocab.gtfs.org/terms#ContinuousAvailable
gtfs:ContinuousAvailable rdf:type owl:NamedIndividual ,
                                  gtfs:ContinuousDropOff ,
                                  gtfs:ContinuousPickup ;
                         rdfs:label "Continuous pickup or drop off is available"@en .


###  http://vocab.gtfs.org/terms#ContinuousNotAvailable
gtfs:ContinuousNotAvailable rdf:type owl:NamedIndividual ,
                                     gtfs:ContinuousDropOff ,
                                     gtfs:ContinuousPickup ;
                            rdfs:label "Continuous pickup or drop off not available"@en .


###  http://vocab.gtfs.org/terms#Elevator
gtfs:Elevator rdf:type owl:NamedIndividual ,
                       gtfs:Pathway .


###  http://vocab.gtfs.org/terms#EnsuredTransfer
gtfs:EnsuredTransfer rdf:type owl:NamedIndividual ,
                              gtfs:TransferType ;
                     rdfs:comment "Este es un punto de transbordo sincronizado entre dos rutas. El vehículo que sale espera al que llega, dejando tiempo suficiente para que un pasajero haga transbordo entre rutas."@es ,
                                  "This is a timed transfer point between two routes. The departing vehicle is expected to wait for the arriving one, with sufficient time for a passenger to transfer between routes."@en ;
                     rdfs:label "Ensured Transfer or Timed Transfer"@en ,
                                "Punto de transbordo sincronizado"@es ;
                     status:term_status "inestable"@es ,
                                        "unstable"@en .


###  http://vocab.gtfs.org/terms#Escalator
gtfs:Escalator rdf:type owl:NamedIndividual ,
                        gtfs:Pathway .


###  http://vocab.gtfs.org/terms#ExitGate
gtfs:ExitGate rdf:type owl:NamedIndividual ,
                       gtfs:Pathway .


###  http://vocab.gtfs.org/terms#FareGate
gtfs:FareGate rdf:type owl:NamedIndividual ,
                       gtfs:Pathway .


###  http://vocab.gtfs.org/terms#Ferry
gtfs:Ferry rdf:type owl:NamedIndividual ,
                    gtfs:RouteType ;
           rdfs:comment "Used for short- and long-distance boat service."@en ,
                        "Utilizado para servicio de transporte público fluvial o marítimo de corta y larga distancia."@es ;
           rdfs:label "Ferry"@en ,
                      "Ferry, transbordador"@es ;
           status:term_status "inestable"@es ,
                              "unstable"@en .


###  http://vocab.gtfs.org/terms#Funicular
gtfs:Funicular rdf:type owl:NamedIndividual ,
                        gtfs:RouteType ;
               rdfs:comment "Any rail system designed for steep inclines."@en ,
                            "Cualquier sistema por raíl diseñado para recorridos con una gran inclinación."@es ;
               rdfs:label "Funicular"@en ,
                          "Funicular"@es ;
               status:term_status "inestable"@es ,
                                  "unstable"@en .


###  http://vocab.gtfs.org/terms#Gondola
gtfs:Gondola rdf:type owl:NamedIndividual ,
                      gtfs:RouteType ;
             rdfs:comment "Gondola, Suspended cable car. Typically used for aerial cable cars where the car is suspended from the cable."@en ,
                          "Normalmente se utiliza para medios de transporte público por cable en donde el vehículo queda suspendido de un cable."@es ;
             rdfs:label "Gondola, Suspended cable car"@en ,
                        "Teleférico, telecabina"@es ;
             owl:deprecated "true" ;
             status:term_status "inestable"@es ,
                                "unstable"@en .


###  http://vocab.gtfs.org/terms#LightRail
gtfs:LightRail rdf:type owl:NamedIndividual ,
                        gtfs:RouteType ;
               rdfs:comment "Any light rail or street level system within a metropolitan area."@en ,
                            "Cualquier metro ligero o sistema ferroviario en superficie dentro de un área metropolitana."@es ;
               rdfs:label "Tram, Streetcar, Light rail"@en ,
                          "Tranvía, metro ligero"@es ;
               status:term_status "inestable"@es ,
                                  "unstable"@en .


###  http://vocab.gtfs.org/terms#MinimumTimeTransfer
gtfs:MinimumTimeTransfer rdf:type owl:NamedIndividual ,
                                  gtfs:TransferType ;
                         rdfs:comment "Este transbordo requiere una cantidad mínima de tiempo entre la llegada y la salida para garantizar la conexión. El tiempo necesario para el transbordo se especifica mediante min_transfer_time"@es ,
                                      "This transfer requires a minimum amount of time between arrival and departure to ensure a connection. The time required to transfer is specified by gtfs:minimumTransferTime"@en ;
                         rdfs:label "Minimum Time Transfer"@en ,
                                    "Mínimo tiempo de transbordo"@es ;
                         status:term_status "inestable"@es ,
                                            "unstable"@en .


###  http://vocab.gtfs.org/terms#Monorail
gtfs:Monorail rdf:type owl:NamedIndividual ,
                       gtfs:RouteType ;
              rdfs:comment "Railway in which the track consists of a single rail or a beam."@en ;
              rdfs:label "Monorail"@en .


###  http://vocab.gtfs.org/terms#MovingSidewalk
gtfs:MovingSidewalk rdf:type owl:NamedIndividual ,
                             gtfs:Pathway .


###  http://vocab.gtfs.org/terms#MustCoordinateWithDriver
gtfs:MustCoordinateWithDriver rdf:type owl:NamedIndividual ,
                                       gtfs:SingleDropOff ,
                                       gtfs:SinglePickup ;
                              rdfs:label "Must coordinate with driver to arrange pickup or drop off"@en ,
                                         "Se debe pedir al conductor que pare."@es ;
                              status:term_status "inestable"@es ,
                                                 "unstable"@en .


###  http://vocab.gtfs.org/terms#MustCoordinateWithDriverForContinuous
gtfs:MustCoordinateWithDriverForContinuous rdf:type owl:NamedIndividual ,
                                                    gtfs:ContinuousDropOff ,
                                                    gtfs:ContinuousPickup ;
                                           rdfs:label "Must coordinate with driver to arrange continuous pickup or drop off"@en .


###  http://vocab.gtfs.org/terms#MustPhone
gtfs:MustPhone rdf:type owl:NamedIndividual ,
                        gtfs:SingleDropOff ,
                        gtfs:SinglePickup ;
               rdfs:label "Must phone agency to arrange pickup or drop off"@en ,
                          "Se debe llamar a la empresa para organizar la parada."@es ;
               status:term_status "inestable"@es ,
                                  "unstable"@en .


###  http://vocab.gtfs.org/terms#MustPhoneForContinuous
gtfs:MustPhoneForContinuous rdf:type owl:NamedIndividual ,
                                     gtfs:ContinuousDropOff ,
                                     gtfs:ContinuousPickup ;
                            rdfs:label "Must phone agency to arrange continuous pickup or drop off"@en .


###  http://vocab.gtfs.org/terms#NoTransfer
gtfs:NoTransfer rdf:type owl:NamedIndividual ,
                         gtfs:TransferType ;
                rdfs:comment "No es posible realizar transbordos entre rutas en esta ubicación."@es ,
                             "Transfers are not possible between routes at this location."@en ;
                rdfs:label "No Transfer"@en ,
                           "Sin transbordo"@es ;
                status:term_status "inestable"@es ,
                                   "unstable"@en .


###  http://vocab.gtfs.org/terms#NoTransfersAllowed
gtfs:NoTransfersAllowed rdf:type owl:NamedIndividual ,
                                 gtfs:TransfersAllowedType ;
                        rdfs:comment "Indica que el pasajero debe comprar un nuevo billete para realizar un transbordo"@es ,
                                     "Indicate that a passenger should buy a new ticket when transferring"@en ;
                        rdfs:label "No se permiten transbordos"@es ,
                                   "No transfers allowed"@en ;
                        status:term_status "inestable"@es ,
                                           "unstable"@en .


###  http://vocab.gtfs.org/terms#NotAvailable
gtfs:NotAvailable rdf:type owl:NamedIndividual ,
                           gtfs:SingleDropOff ,
                           gtfs:SinglePickup ;
                  rdfs:label "Pickup or drop off not available"@en ,
                             "Sin parada disponible"@es ;
                  status:term_status "inestable"@es ,
                                     "unstable"@en .


###  http://vocab.gtfs.org/terms#NotWheelchairAccessible
gtfs:NotWheelchairAccessible rdf:type owl:NamedIndividual ,
                                      gtfs:WheelchairBoardingStatus ;
                             gtfs:comment "Corresponde a wheelchair_accessible con valor 2"@es ,
                                          "Corresponds to a wheelchair_accessible column being 2"@en ;
                             rdfs:comment "No riders in wheelchairs can be accommodated on this trip or wheelchair boarding is not possible at this stop and/or there exists no accessible path from outside the station to the specific stop."@en ,
                                          "Pasajeros en silla de ruedas no pueden acceder a este viaje o el acceso con silla de ruedas no es posible en esta parada y/o no hay una ruta accesible desde el exterior de la estación hasta la parada."@es ;
                             rdfs:label "No accesible para silla de ruedas"@es ,
                                        "Not wheelchair accessible"@en ;
                             status:term_status "inestable"@es ,
                                                "unstable"@en .


###  http://vocab.gtfs.org/terms#OnBoard
gtfs:OnBoard rdf:type owl:NamedIndividual ,
                      gtfs:PaymentMethod ;
             rdfs:comment "Fare should be bought on board"@en ,
                          "La tarifa se paga a bordo"@es ;
             rdfs:label "A bordo"@es ,
                        "On Board"@en ;
             status:term_status "inestable"@es ,
                                "unstable"@en .


###  http://vocab.gtfs.org/terms#OneTransfersAllowed
gtfs:OneTransfersAllowed rdf:type owl:NamedIndividual ,
                                  gtfs:TransfersAllowedType ;
                         rdfs:comment "Indica que el pasajero puede hacer un transbordo con su billete"@es ,
                                      "Indicate that a passenger should buy a new ticket when transferring a second time"@en ;
                         rdfs:label "One transfer allowed"@en ,
                                    "Un transbordo permitido"@es ;
                         status:term_status "inestable"@es ,
                                            "unstable"@en .


###  http://vocab.gtfs.org/terms#Rail
gtfs:Rail rdf:type owl:NamedIndividual ,
                   gtfs:RouteType ;
          rdfs:comment "Used for intercity or long-distance travel."@en ,
                       "Utilizado para viajes de cercanías, interurbanos o de larga distancia."@es ;
          rdfs:label "Rail"@en ,
                     "Tren"@es ;
          status:term_status "inestable"@es ,
                             "unstable"@en .


###  http://vocab.gtfs.org/terms#RecommendedTransfer
gtfs:RecommendedTransfer rdf:type owl:NamedIndividual ,
                                  gtfs:TransferType ;
                         rdfs:comment "Este es un punto de transbordo recomendado entre dos rutas"@es ,
                                      "This is a recommended transfer point between two routes"@en ;
                         rdfs:label "Punto de transbordo recomendado"@es ,
                                    "Recommended Transfer"@en ;
                         status:term_status "inestable"@es ,
                                            "unstable"@en .


###  http://vocab.gtfs.org/terms#Regular
gtfs:Regular rdf:type owl:NamedIndividual ,
                      gtfs:SingleDropOff ,
                      gtfs:SinglePickup ;
             gtfs:comment "If no pickup_type or drop_off_type given in stop_times.txt, map to this one."@en ,
                          "Si no se incluye pickup_type o drop_off_type en stop_times.txt, mapee a este concepto."@es ;
             rdfs:label "Parada programada regularmente"@es ,
                        "Regularly scheduled pickup or drop off"@en ;
             status:term_status "inestable"@es ,
                                "unstable"@en .


###  http://vocab.gtfs.org/terms#Stairs
gtfs:Stairs rdf:type owl:NamedIndividual ,
                     gtfs:Pathway .


###  http://vocab.gtfs.org/terms#Subway
gtfs:Subway rdf:type owl:NamedIndividual ,
                     gtfs:RouteType ;
            rdfs:comment "Any underground rail system within a metropolitan area."@en ,
                         "Cualquier sistema ferroviario subterráneo dentro de un área metropolitana."@es ;
            rdfs:label "Subterráneo, metro"@es ,
                       "Subway, Metro"@en ;
            status:term_status "inestable"@es ,
                               "unstable"@en .


###  http://vocab.gtfs.org/terms#Trolleybus
gtfs:Trolleybus rdf:type owl:NamedIndividual ,
                         gtfs:RouteType ;
                rdfs:comment "Electric buses that draw power from overhead wires using poles."@en ;
                rdfs:label "Trolleybus"@en .


###  http://vocab.gtfs.org/terms#TwoTransfersAllowed
gtfs:TwoTransfersAllowed rdf:type owl:NamedIndividual ,
                                  gtfs:TransfersAllowedType ;
                         rdfs:comment "Indica que el pasajero puede hacer dos transbordos con su billete"@es ,
                                      "Indicate that a passenger should buy a new ticket when transferring for the third time"@en ;
                         rdfs:label "Dos transbordos permitidos"@es ,
                                    "Two transfers allowed"@en ;
                         status:term_status "inestable"@es ,
                                            "unstable"@en .


###  http://vocab.gtfs.org/terms#UnlimitedTransfersAllowed
gtfs:UnlimitedTransfersAllowed rdf:type owl:NamedIndividual ,
                                        gtfs:TransfersAllowedType ;
                               rdfs:comment "Indica que el billete permite una cantidad de transbordos ilimitada"@es ,
                                            "Indicate that unlimited transfers are permitted"@en ;
                               rdfs:label "Transbordos ilimitados"@es ,
                                          "Unlimited transfers allowed"@en ;
                               status:term_status "inestable"@es ,
                                                  "unstable"@en .


###  http://vocab.gtfs.org/terms#Walkway
gtfs:Walkway rdf:type owl:NamedIndividual ,
                      gtfs:Pathway .


###  http://vocab.gtfs.org/terms#WheelchairAccessible
gtfs:WheelchairAccessible rdf:type owl:NamedIndividual ,
                                   gtfs:WheelchairBoardingStatus ;
                          gtfs:comment "Corresponde a wheelchair_accessible con valor 1"@es ,
                                       "Corresponds to a wheelchair_accessible column being 1"@en ;
                          rdfs:comment "Indica que el vehículo usado en este viaje es accesible para, al menos, un pasajero en silla de ruedas, o indica que la parada específica está habilitada para sillas de ruedas, que algunos viajes desde esta parada son accesibles para silla de ruedas y si esta parada tiene una estación matriz, que hay alguna ruta accesible desde el exterior de la estación hasta la parada."@es ,
                                       "Indicates that the vehicle being used on this particular trip can accommodate at least one rider in a wheelchair, or identifies that wheelchair boardings are possible from the specified stop, some trips at this stop are accessible by wheelchair and if this stop has a parentStation, there exists some accessible path from outside the station to the specific stop."@en ;
                          rdfs:label "Accesible para silla de ruedas"@es ,
                                     "Wheelchair accessible"@en ;
                          status:term_status "inestable"@es ,
                                             "unstable"@en .


[ foaf:mbox "Pieter.Colpaert@UGent.be" ;
  foaf:name "Pieter Colpaert"
] .

[ foaf:mbox "abyrd@conveyal.com" ;
   foaf:name "Andrew Byrd"
 ] .

#################################################################
#    Annotations
#################################################################

gtfs:Elevator rdfs:label "Elevator"@en .


gtfs:Escalator rdfs:label "Escalator"@en .


gtfs:ExitGate rdfs:label "Exit Gate"@en ;
              rdfs:comment "Indicates a pathway exiting an area where proof-of-payment is required into an area where proof-of-payment is no longer required."@en .


gtfs:FareGate rdfs:comment "A pathway that crosses into an area of the station where a proof of payment is required (usually via a physical payment gate). Fare gates may either separate paid areas of the station from unpaid ones, or separate different payment areas within the same station from each other. This information can be used to avoid routing passengers through stations using shortcuts that would require passengers to make unnecessary payments, like directing a passenger to walk through a subway platform to reach a busway."@en ;
              rdfs:label "Fare Gate"@en .


gtfs:MovingSidewalk rdfs:label "Moving Sidewalk or Travelator"@en .


gtfs:Stairs rdfs:label "Stairs"@en .


gtfs:Walkway rdfs:label "Walkway"@en .


gtfs:destinationZone rdfs:label "Destination Zone"@en ;
                     status:term_status "unstable"@en ;
                     rdfs:comment "La zona de destino donde una clase tarifaria se aplica"@en ;
                     rdfs:label "zona de destino"@es ;
                     rdfs:comment "The destination zone where this applies"@en ;
                     status:term_status "inestable"@es .


gtfs:originZone rdfs:label "zona de origen"@es ;
                status:term_status "inestable"@es ;
                rdfs:label "Origin Zone"@en ;
                status:term_status "unstable"@en ;
                rdfs:comment "La zona de origen donde una clase tarifaria se aplica"@es ,
                             "The origin zone where this applies"@en .


gtfs:transferExpiryTime rdfs:label "Transfer Expiry Time"@en ;
                        status:term_status "inestable"@es ;
                        rdfs:label "Tiempo de validez para el transbordo"@es ;
                        rdfs:comment "El tiempo que el billete es válido desde que se abandona el vehículo para hacer un transbordo"@es ;
                        status:term_status "unstable"@en ;
                        rdfs:comment "The time a ticket remains valid when having left the previous vehicle"@en .


gtfs:translation rdfs:comment "Links the entity to its translation."@en ;
                 rdfs:label "Translation"@en .


###  Generated by the OWL API (version 4.5.9.2019-02-01T07:24:44Z) https://github.com/owlcs/owlapi
